theories/examples/awkward_example.v
@@ -619,6 +619,8 @@ Section awkward_example.
    (* assume r1 contains an executable pointer to adversarial code *)
   (* assume r0 contains an executable pointer to the awkward example *)
   Definition awkward_instrs (r1 : RegName) epilogue_off :=
+     reqglob_instrs r1 ++
+     prepstack_instrs r_stk 11 ++
      [store_z r_env 0] ++
      push_r_instrs r_stk r_env ++
      push_r_instrs r_stk r_t0 ++
@@ -1492,12 +1494,12 @@ Section awkward_example.
 
    (* the following spec is for the f4 subroutine of the awkward example, jumped to after dynamically allocating into r_env *)
   Lemma f4_spec W pc_p pc_g pc_b pc_e (* PC *)
-        b e a (* adv *)
-        g_ret b_ret e_ret a_ret (* return cap *)
+        wadv (* b e a *) (* adv *)
+        wret (* g_ret b_ret e_ret a_ret *) (* return cap *)
         f4_addrs (* f2 *)
         d d' i (* dynamically allocated memory given by preamble, connected to invariant i *)
         a_first a_last (* special adresses *) 
-        (b_r e_r b_r' : Addr) (* stack *)
+        wstk (* (b_r e_r b_r' : Addr) *) (* stack *)
         rmap (* registers *) :
 
     (* PC assumptions *)
@@ -1507,8 +1509,8 @@ Section awkward_example.
     contiguous_between f4_addrs a_first a_last ->
     
     (* Stack assumptions *)
-    region_size b_r e_r > 11 -> (* we must assume the stack is large enough for needed local state *)
-    (b_r' + 1)%a = Some b_r ->
+    (* region_size b_r e_r > 11 -> (* we must assume the stack is large enough for needed local state *) *)
+    (* (b_r' + 1)%a = Some b_r -> *)
 
     (* malloc'ed memory assumption *)
     (d + 1)%a = Some d' ->
@@ -1518,27 +1520,27 @@ Section awkward_example.
 
     (* Finally, we must assume that the stack is currently in a temporary state *)
     (* (forall (a : Addr), W.1.1 !! (encode a) = Some (encode Temporary) <-> a ∈ (region_addrs b_r e_r)) -> *)
-    Forall (λ a, region_type_temporary W a) (region_addrs b_r e_r) ->
+    (* Forall (λ a, region_type_temporary W a) (region_addrs b_r e_r) -> *)
 
-    {{{ r_stk ↦ᵣ inr ((RWLX,Local),b_r,e_r,b_r')
+    {{{ r_stk ↦ᵣ wstk
       ∗ PC ↦ᵣ inr ((pc_p,pc_g),pc_b,pc_e,a_first)
-      ∗ r_t0 ↦ᵣ inr ((E,g_ret),b_ret,e_ret,a_ret) (* for now we say it's an enter cap. We will need to generalize to all words *)
-      ∗ r_adv ↦ᵣ inr ((E,Global),b,e,a)
+      ∗ r_t0 ↦ᵣ wret
+      ∗ r_adv ↦ᵣ wadv
       ∗ r_env ↦ᵣ inr (RWX,Global,d,d',d)
       ∗ ([∗ map] r_i↦w_i ∈ rmap, r_i ↦ᵣ w_i)
       (* invariant for d *)
       ∗ (∃ ι, inv ι (awk_inv i d))
       ∗ sts_rel_loc (A:=Addr) i awk_rel_pub awk_rel_priv
       (* stack *)
-      ∗ ([∗ list] a ∈ (region_addrs b_r e_r), rel a RWLX (λ Wv : WORLD * Word, (interp Wv.1) Wv.2))
+      ∗ interp W wstk
       (* token which states all non atomic invariants are closed *)
       ∗ na_own logrel_nais ⊤
       (* adv code *)
-      ∗ ([∗ list] a ∈ (region_addrs b e), (read_write_cond a RX interp) ∧ ⌜region_state_nwl W a Global⌝)
+      ∗ interp W wadv
       (* callback validity *)
-      ∗ interp W (inr ((E,g_ret),b_ret,e_ret,a_ret))
+      ∗ interp W wret
       (* trusted code *)
-      ∗ awkward_example f4_addrs pc_p r_adv 65
+      ∗ (∃ ι, na_inv logrel_nais ι (awkward_example f4_addrs pc_p r_adv 65))
       (* we start out with arbitrary sts *)
       ∗ sts_full_world W
       ∗ region W
@@ -1551,15 +1553,69 @@ Section awkward_example.
                          ∗ sts_full_world W'
                          ∗ region W' }}}.
   Proof.
-    iIntros (Hvpc Hf2 Hsize Hb_r' Hd Hrmap_dom Htemp φ)
+    iIntros (Hvpc Hcont Hd Hrmap_dom φ)
             "(Hr_stk & HPC & Hr_t0 & Hr_adv & Hr_env & Hgen_reg & #Hι & #Hrel & #Hstack_val & Hna & #Hadv_val & #Hcallback & Hprog & Hsts & Hr) Hφ".
-    (* We put the code in a non atomic invariant for each iteration of the program *)
-    iMod (na_inv_alloc logrel_nais ⊤ (nroot.@"prog") with "Hprog") as "#Hf4".
+    iDestruct "Hprog" as (ιprog) "#Hf4". 
     (* Now we step through the program *)
     iMod (na_inv_open with "Hf4 Hna") as "(>Hprog & Hna & Hcls)";[auto..|]. 
     iDestruct (big_sepL2_length with "Hprog") as %Hprog_length.
     destruct (f4_addrs);[inversion Hprog_length|].
-    iDestruct "Hι" as (ι) "Hinv". 
+    iDestruct "Hι" as (ι) "Hinv".
+    (* We get some general purpose registers *)
+    iAssert ((∃ w1, r_t1 ↦ᵣ w1) ∗ (∃ w2, r_t2 ↦ᵣ w2) ∗ [∗ map] r_i↦w_i ∈ delete r_t2 (delete r_t1 rmap), r_i ↦ᵣ w_i)%I
+      with "[Hgen_reg]" as "(Hr_t1 & Hr_t2 & Hgen_reg)".
+    { assert (is_Some (rmap !! r_t1)) as [w1 Hrt1].
+      { apply elem_of_gmap_dom. rewrite Hrmap_dom. apply elem_of_difference.
+        split;[apply all_registers_s_correct|clear;set_solver]. }
+      assert (is_Some (delete r_t1 rmap !! r_t2)) as [w2 Hrt2].
+      { apply elem_of_gmap_dom. rewrite dom_delete_L Hrmap_dom. apply elem_of_difference.
+        split;[|clear;set_solver]. apply elem_of_difference.
+        split;[apply all_registers_s_correct|clear;set_solver]. }
+      iDestruct (big_sepM_delete _ _ r_t1 with "Hgen_reg") as "[Hr_t1 Hgen_reg]";[eauto|].
+      iDestruct (big_sepM_delete _ _ r_t2 with "Hgen_reg") as "[Hr_t2 Hgen_reg]";[eauto|].
+      iSplitL "Hr_t1";[eauto|]. iSplitL "Hr_t2";[eauto|]. iFrame. 
+    }
+    (* First we require wadv to be global *)
+    iDestruct (contiguous_between_program_split with "Hprog") as (reqperm_prog rest link)
+                                                                   "(Hreqglob & Hprog & #Hcont)";[apply Hcont|].
+    iDestruct "Hcont" as %(Hcont_reqglob & Hcont_rest & Heqapp & Hlink).
+    iDestruct (big_sepL2_length with "Hreqglob") as %Hreqglob_length. simpl in Hreqglob_length. 
+    iApply (reqglob_spec with "[-]");
+      [|apply PermFlows_refl|apply Hcont_reqglob|iFrame "HPC Hreqglob Hr_adv Hr_t1 Hr_t2"]. 
+    { intros mid Hmid. apply isCorrectPC_inrange with a_first a_last; auto.
+      apply contiguous_between_bounds in Hcont_rest. revert Hmid Hcont_rest;clear;solve_addr. }
+    iNext. destruct (isGlobalWord wadv) eqn:Hglob;[|(* Failure *) iApply "Hφ";iIntros (Hcontr);inversion Hcontr].
+    (* If the macro is successful, we can infer that it is a Global capability *)
+    destruct wadv as [z | [ [ [ [p g] b] e] a'] ];[inversion Hglob|].
+    destruct g;[|inversion Hglob]. iExists _,_,_,_. iSplit;[eauto|]. iIntros "(HPC & Hreqglob & Hr_adv & Hr_t1 & Hr_t2)".
+    (* Next we prepare the stack *)
+    iDestruct (contiguous_between_program_split with "Hprog") as (preptack_prog rest0 link0)
+                                                                   "(Hprepstack & Hprog & #Hcont)";[apply Hcont_rest|].
+    iDestruct "Hcont" as %(Hcont_prepstack & Hcont_rest0 & Heqapp0 & Hlink0).
+    iDestruct (big_sepL2_length with "Hprepstack") as %Hprepstack_length. simpl in Hprepstack_length. 
+    iApply (prepstack_spec with "[-]");
+      [|apply PermFlows_refl|apply Hcont_prepstack|iFrame "HPC Hprepstack Hr_stk"].
+    { intros mid Hmid. apply isCorrectPC_inrange with a_first a_last; auto.
+      apply contiguous_between_bounds in Hcont_rest0. revert Hmid Hcont_rest0 Hlink;clear. solve_addr. }
+    iSplitL "Hr_t1";[iNext;eauto|]. iSplitL "Hr_t2";[iNext;eauto|].
+    iNext. destruct (isPermWord wstk RWLX) eqn:Hperm;[|(* Failure *) iApply "Hφ";iIntros (Hcontr);inversion Hcontr].
+    destruct (11 <? cap_size wstk)%Z eqn:Hsize';[|(* Failure *) iApply "Hφ";iIntros (Hcontr);inversion Hcontr].
+    destruct (decide (is_Some (bound_check wstk)))%Z;[|(* Failure *) iApply "Hφ";iIntros (Hcontr);inversion Hcontr].
+    iIntros "Hcont".
+    iDestruct "Hcont" as (l0 b_r e_r a_r' b_r' Heq Hb_r') "(HPC & Hprestack & Hr_stk & Hr_t1 & Hr_t2)".
+    (* We cleanup our definitions *)
+    simplify_eq.
+    assert (region_size b_r e_r > 11) as Hsize;[|clear Hperm i0 Hsize'].
+    { apply Zlt_is_lt_bool in Hsize'. revert Hsize'. clear. rewrite /region_size /=. lia. }
+    (* If the stack is Global, validity is false *)
+    destruct l0;[by rewrite fixpoint_interp1_eq;iSimpl in "Hstack_val"|].
+    rewrite fixpoint_interp1_eq;iSimpl in "Hstack_val".
+    iDestruct "Hstack_val" as (p0 Hperm) "[Hstack_region _]". destruct p0;inversion Hperm. clear Hperm.
+    iAssert (⌜Forall (λ a, region_type_temporary W a) (region_addrs b_r e_r)⌝)%I as %Htemp.
+    { iDestruct (big_sepL_and with "Hstack_region") as "[Hstack_rel Hstack_pwl]".
+      iDestruct (big_sepL_forall with "Hstack_pwl") as %Hforall.
+      iPureIntro. rewrite Forall_forall. intros x Hin. apply elem_of_list_lookup_1 in Hin as [k Hin].
+      apply Hforall in Hin. auto. }
     (* We will now need to open the invariant for d. 
        We do not know which state d is in, and may need to 
        do a private transition from 1 to 0! For that reason 
@@ -1573,7 +1629,8 @@ Section awkward_example.
     { iSplit.
       - iApply big_sepL_forall. iPureIntro. intros n. simpl. intros x Hsome. apply Hiff. apply elem_of_app; left.
         apply elem_of_list_lookup. eauto. 
-      - iApply (big_sepL_mono with "Hstack_val"). iIntros (k y Hk) "Hrel". iFrame. iPureIntro.
+      - iApply (big_sepL_mono with "Hstack_region"). iIntros (k y Hk) "[Hrel _]". rewrite /read_write_cond.
+        iFrame. iPureIntro.
         revert Htemp; rewrite Forall_forall =>Htemp. apply Htemp. apply elem_of_list_lookup. eauto. }
     iAssert ((▷ ∃ ws, [[b_r, e_r]]↦ₐ[RWLX][[ws]])
                ∗ ⌜Forall (λ a : Addr, region_type_revoked (revoke W) a) (region_addrs b_r e_r)⌝)%I
@@ -1594,13 +1651,18 @@ Section awkward_example.
        say that there exists some private future world such that   
        the store succeeded, after which the state at i is false
      *)
-    iPrologue l Hprog_length "Hprog".
-    apply contiguous_between_cons_inv_first in Hf2 as Heq. subst a_first. 
+    iDestruct (big_sepL2_length with "Hprog") as %Hrest0_length.
+    destruct rest0;[inversion Hrest0_length|]. 
+    iPrologue rest0 Hrest0_length "Hprog".
+    apply contiguous_between_cons_inv_first in Hcont_rest0 as Heq. subst a0.
+    assert (isCorrectPC_range pc_p pc_g pc_b pc_e link0 a_last) as Hvpc'.
+    { intros mid Hmid. apply isCorrectPC_inrange with a_first a_last; auto.
+      revert Hlink Hlink0 Hmid. clear. solve_addr. }
     assert (withinBounds (RWX, Global, d, d', d) = true) as Hwb.
     { isWithinBounds;[lia|]. revert Hd; clear. solve_addr. }
     iAssert (▷ (PC ↦ᵣ inr (pc_p, pc_g, pc_b, pc_e, a1)
               ∗ r_env ↦ᵣ inr (RWX, Global, d, d', d)
-              ∗ a0 ↦ₐ[pc_p] store_z r_env 0
+              ∗ link0 ↦ₐ[pc_p] store_z r_env 0
               ∗ (∃ W',⌜(∃ b : bool, W.2.1 !! i = Some (encode b))
                         ∧ W.2.2 !! i = Some (convert_rel awk_rel_pub, convert_rel awk_rel_priv)⌝ ∧ 
                     ⌜W' = ((revoke_std_sta W.1),(<[i:=encode false]> W.2.1,W.2.2))⌝ ∧
@@ -1616,7 +1678,7 @@ Section awkward_example.
       iInv ι as (x) "[>Hstate Hb]" "Hcls".
       destruct x; iDestruct "Hb" as ">Hb".
       - iApply (wp_store_success_z with "[$HPC $Hinstr $Hr_env $Hb]");
-          [apply store_z_i|apply PermFlows_refl|apply PermFlows_refl|iCorrectPC a0 a_last|iContiguous_next Hf2 0|auto|auto|..].
+          [apply store_z_i|apply PermFlows_refl|apply PermFlows_refl|iCorrectPC link0 a_last|iContiguous_next Hcont_rest0 0|auto|auto|..].
         iNext. iIntros "(HPC & Hinstr & Hr_env & Hd)".
         (* we assert that updating the local state d to 0 is a private transition *)
         iDestruct (sts_full_state_loc with "Hsts Hstate") as %Hlookup.
@@ -1645,7 +1707,7 @@ Section awkward_example.
         eapply Forall_impl;[apply Hrevoked|].
         intros a2 Ha0_rev; auto. 
       - iApply (wp_store_success_z with "[$HPC $Hinstr $Hr_env $Hb]");
-          [apply store_z_i|apply PermFlows_refl|apply PermFlows_refl|iCorrectPC a0 a_last|iContiguous_next Hf2 0|auto|auto|..].
+          [apply store_z_i|apply PermFlows_refl|apply PermFlows_refl|iCorrectPC link0 a_last|iContiguous_next Hcont_rest0 0|auto|auto|..].
         iNext. iIntros "(HPC & Hinstr & Hr_env & Hd)".
         (* use sts_state to assert that the current state of i is false *)
         iDestruct (sts_full_state_loc with "Hsts Hstate") as %Hlookup.
@@ -1678,9 +1740,9 @@ Section awkward_example.
            by exists [w;w0;w1;w2;w3;w4;w5;w6;w7;w8;w9],ws. }
     rewrite Happ.
     iDestruct (contiguous_between_program_split with "Hstack") as (stack_own stack_adv stack_own_last) "(Hstack_own & Hstack_adv & #Hcont)"; [eauto|].
-    iDestruct "Hcont" as %(Hcont1 & Hcont2 & Hstack_eq & Hlink).
+    iDestruct "Hcont" as %(Hcont1 & Hcont2 & Hstack_eq1 & Hlink1).
     iDestruct (big_sepL2_length with "Hstack_own") as %Hlength_own. rewrite Hlength' in Hlength_own.
-    rewrite Hstack_eq in Hcontiguous.
+    rewrite Hstack_eq1 in Hcontiguous.
     (* The following length assumptions will let us destruct the stack/program *)
     iDestruct (big_sepL2_length with "Hprog") as %Hlength_f2.
     iDestruct (big_sepL2_length with "Hstack_adv") as %Hlength_adv.
@@ -1688,42 +1750,42 @@ Section awkward_example.
     do 3 (destruct stack_own; [inversion Hlength_own|]; destruct ws_own;[inversion Hlength'|]).
     assert ((region_addrs b_r e_r) !! 0 = Some b_r) as Hfirst_stack.
     { apply region_addrs_first. revert Hsize; clear. rewrite /region_size. solve_addr. }
-    rewrite Hstack_eq /= in Hfirst_stack. inversion Hfirst_stack as [Heq]. subst b_r.
+    rewrite Hstack_eq1 /= in Hfirst_stack. inversion Hfirst_stack as [Heq]. subst b_r.
     (* assert that the stack bounds are within bounds *)
-    assert (withinBounds (RWLX,Local,a2,e_r,a2) = true ∧ withinBounds (RWLX,Local,a2,e_r,stack_own_last) = true) as [Hwb1 Hwb2].
+    assert (withinBounds (RWLX,Local,a0,e_r,a0) = true ∧ withinBounds (RWLX,Local,a0,e_r,stack_own_last) = true) as [Hwb1 Hwb2].
     { split; isWithinBounds; first lia.
       - revert Hlength. rewrite Happ app_length Hlength' region_addrs_length /region_size. clear. solve_addr.
       - by eapply contiguous_between_bounds.
       - apply contiguous_between_bounds in Hcont2. simplify_eq.
-        revert Hlength' Hlength Hlink Hsize Hlength_adv Hlength_own Hcont2. rewrite -region_addrs_length app_length. clear.
+        revert Hlength' Hlength Hlink1 Hsize Hlength_adv Hlength_own Hcont2. rewrite -region_addrs_length app_length. clear.
         rewrite region_addrs_length /region_size. solve_addr.
     }   
     (* push r_stk r_env *)
     iDestruct "Hstack_own" as "[Ha Hstack_own]".
-    do 2 (destruct l;[inversion Hprog_length|]).
-    iDestruct (big_sepL2_app_inv _ [a1;a5] (a6::l) with "Hprog") as "[Hpush Hprog]";[simpl;auto|]. 
+    do 2 (destruct rest0;[inversion Hrest0_length|]).
+    iDestruct (big_sepL2_app_inv _ [a1;a4] (a5::rest0) with "Hprog") as "[Hpush Hprog]";[simpl;auto|]. 
     iApply (push_r_spec);[..|iFrame "HPC Hr_stk Hpush Hr_env Ha"];
-      [|apply PermFlows_refl|auto|iContiguous_next Hf2 1|iContiguous_next Hf2 2|auto|..].
-    { split;iCorrectPC a0 a_last. }
+      [|apply PermFlows_refl|auto|iContiguous_next Hcont_rest0 1|iContiguous_next Hcont_rest0 2|auto|..].
+    { split;iCorrectPC link0 a_last. }
     iNext. iIntros "(HPC & Hpush & Hr_stk & Hr_env & Hb_r)". iCombine "Hpush" "Hprog_done" as "Hprog_done".
     (* push r_stk r_self *)
-    do 2 (destruct l;[inversion Hprog_length|]).
-    iDestruct (big_sepL2_app_inv _ [a6;a7] (a8::l) with "Hprog") as "[Hpush Hprog]";[simpl;auto|]. 
+    do 2 (destruct rest0;[inversion Hrest0_length|]).
+    iDestruct (big_sepL2_app_inv _ [a5;a6] (a7::rest0) with "Hprog") as "[Hpush Hprog]";[simpl;auto|]. 
     iDestruct "Hstack_own" as "[Ha2 Hstack_own]".
     iApply (push_r_spec);[..|iFrame "HPC Hr_stk Hpush Hr_t0 Ha2"];
-      [|apply PermFlows_refl| |iContiguous_next Hf2 3|
-       iContiguous_next Hf2 4|iContiguous_next Hcont1 0|..].
-    { split;iCorrectPC a0 a_last. }
-    { iContiguous_bounds_withinBounds a2 stack_own_last. }
+      [|apply PermFlows_refl| |iContiguous_next Hcont_rest0 3|
+       iContiguous_next Hcont_rest0 4|iContiguous_next Hcont1 0|..].
+    { split;iCorrectPC link0 a_last. }
+    { iContiguous_bounds_withinBounds a0 stack_own_last. }
     iNext. iIntros "(HPC & Hpush & Hr_stk & Hr_self & Ha2)". iCombine "Hpush" "Hprog_done" as "Hprog_done".
     (* push r_stk r_adv *)
-    do 2 (destruct l;[inversion Hprog_length|]).
-    iDestruct (big_sepL2_app_inv _ [a8;a9] (a10::l) with "Hprog") as "[Hpush Hprog]";[simpl;auto|].
+    do 2 (destruct rest0;[inversion Hrest0_length|]).
+    iDestruct (big_sepL2_app_inv _ [a7;a8] (a9::rest0) with "Hprog") as "[Hpush Hprog]";[simpl;auto|].
     iDestruct "Hstack_own" as "[Ha3 Hstack_own]".
     iApply (push_r_spec);[..|iFrame "HPC Hr_stk Hpush Hr_adv Ha3"];
-      [|apply PermFlows_refl|iContiguous_bounds_withinBounds a2 stack_own_last|iContiguous_next Hf2 5|
-       iContiguous_next Hf2 6|iContiguous_next Hcont1 1|..].
-    { split;iCorrectPC a0 a_last. }
+      [|apply PermFlows_refl|iContiguous_bounds_withinBounds a0 stack_own_last|iContiguous_next Hcont_rest0 5|
+       iContiguous_next Hcont_rest0 6|iContiguous_next Hcont1 1|..].
+    { split;iCorrectPC link0 a_last. }
     iNext. iIntros "(HPC & Hpush & Hr_stk & Hr_adv & Ha3)". iCombine "Hpush" "Hprog_done" as "Hprog_done".
     (* prepare for scall *)
     (* Prepare the scall prologue macro *)
@@ -1733,70 +1795,59 @@ Section awkward_example.
       repeat (inversion Hcont1 as [|????? Hcont1']; subst; auto; clear Hcont1; rename Hcont1' into Hcont1). }      
     assert (stack_adv = region_addrs stack_own_last e_r) as ->.
     { apply region_addrs_of_contiguous_between; auto. }
-    assert (contiguous_between (a10 :: l) a10 a_last) as Hcont_weak.
-    { repeat (inversion Hf2 as [|????? Hf2']; subst; auto; clear Hf2; rename Hf2' into Hf2). }
-    iDestruct (contiguous_between_program_split with "Hprog") as (scall_prologue rest0 s_last)
+    assert (contiguous_between (a9 :: rest0) a9 a_last) as Hcont_weak.
+    { repeat (inversion Hcont_rest0 as [|????? Hcont_rest0']; subst; auto; clear Hcont_rest0; rename Hcont_rest0' into Hcont_rest0). }
+    iDestruct (contiguous_between_program_split with "Hprog") as (scall_prologue rest1 s_last)
                                                                    "(Hscall & Hf2 & #Hcont)"; [eauto|..].
     clear Hfirst_stack Hcont_weak.
-    iDestruct "Hcont" as %(Hcont_scall & Hcont_rest0 & Hrest_app & Hlink').
+    iDestruct "Hcont" as %(Hcont_scall & Hcont_rest1 & Hrest_app & Hlink').
     iDestruct (big_sepL2_length with "Hscall") as %Hscall_length. simpl in Hscall_length, Hlength_f2.
     assert ((stack_own_b + 8)%a = Some stack_own_last) as Hstack_own_bound.
-    { rewrite -(addr_add_assoc a2 _ 3). assert ((3 + 8) = 11)%Z as ->;[done|].
-      rewrite Hlength_own in Hlink. revert Hlink; clear; solve_addr.
+    { rewrite -(addr_add_assoc a0 _ 3). assert ((3 + 8) = 11)%Z as ->;[done|].
+      rewrite Hlength_own in Hlink1. revert Hlink1; clear; solve_addr.
       apply contiguous_between_incr_addr with (i:=3) (ai:=stack_own_b) in Hcont1; auto. }
     assert (∃ a, (stack_own_b + 7)%a = Some a) as [stack_own_end Hstack_own_bound'].
     { revert Hstack_own_bound. clear. intros H. destruct (stack_own_b + 7)%a eqn:Hnone; eauto. solve_addr. }
-    assert (a10 < s_last)%a as Hcontlt.
+    assert (a9 < s_last)%a as Hcontlt.
     { revert Hscall_length Hlink'. clear. solve_addr. }
-    assert (a0 <= a10)%a as Hcontge.
-    { apply region_addrs_of_contiguous_between in Hcont_scall. simplify_eq. revert Hscall_length Hf2 Hcontlt. clear =>Hscall_length Hf2 Hcontlt.
-      apply contiguous_between_middle_bounds with (i := 7) (ai := a10) in Hf2;[solve_addr|auto]. 
+    assert (link0 <= a9)%a as Hcontge.
+    { apply region_addrs_of_contiguous_between in Hcont_scall. simplify_eq. revert Hscall_length Hcont_rest0 Hcontlt. clear =>Hscall_length Hf2 Hcontlt.
+      apply contiguous_between_middle_bounds with (i := 7) (ai := a9) in Hf2;[solve_addr|auto]. 
     }
     (* scall *)
+    iDestruct (big_sepM_insert _ _ r_t1 with "[$Hgen_reg $Hr_t1]") as "Hgen_reg".
+    { rewrite lookup_delete_ne;auto. apply lookup_delete. }
+    iDestruct (big_sepM_insert _ _ r_t2 with "[$Hgen_reg $Hr_t2]") as "Hgen_reg".
+    { rewrite lookup_insert_ne;auto. apply lookup_delete. }
     iDestruct (big_sepM_insert _ _ r_env with "[$Hgen_reg $Hr_env]") as "Hgen_reg".
-    { enough (r_env ∉ dom (gset RegName) rmap) as HH by rewrite not_elem_of_dom // in HH.
+    { repeat (try rewrite lookup_insert_ne;auto; try rewrite lookup_delete_ne;auto). 
+      enough (r_env ∉ dom (gset RegName) rmap) as HH by rewrite not_elem_of_dom // in HH.
       rewrite Hrmap_dom. rewrite not_elem_of_difference; right. set_solver. }
     iDestruct (big_sepM_insert _ _ r_t0 with "[$Hgen_reg $Hr_self]") as "Hgen_reg".
-    { rewrite lookup_insert_ne //.
+    { repeat (try rewrite lookup_insert_ne;auto; try rewrite lookup_delete_ne;auto). 
       enough (r_t0 ∉ dom (gset RegName) rmap) as HH by rewrite not_elem_of_dom // in HH.
       rewrite Hrmap_dom. rewrite not_elem_of_difference; right. set_solver. }
     iApply (scall_prologue_spec with "[- $HPC $Hr_stk $Hscall $Hstack_own $Hstack_adv $Hgen_reg]");
       [ | | apply Hwb2|apply Hcont_scall|apply PermFlows_refl|iNotElemOfList| |
         iContiguous_next Hcont1 2|apply Hstack_own_bound'|apply Hstack_own_bound| |done|..].
-    { assert (s_last <= a_last)%a as Hle;[by apply contiguous_between_bounds in Hcont_rest0|].
-      intros mid Hmid. apply isCorrectPC_inrange with a0 a_last; auto.
+    { assert (s_last <= a_last)%a as Hle;[by apply contiguous_between_bounds in Hcont_rest1|].
+      intros mid Hmid. apply isCorrectPC_inrange with link0 a_last; auto.
       revert Hle Hcontlt Hcontge Hmid. clear. intros. split; solve_addr. }
-    { simplify_eq. iContiguous_bounds_withinBounds a2 stack_own_last. }
-    { rewrite !dom_insert_L Hrmap_dom !singleton_union_difference_L !all_registers_union_l.
+    { simplify_eq. iContiguous_bounds_withinBounds a0 stack_own_last. }
+    { rewrite !dom_insert_L !dom_delete_L !Hrmap_dom !singleton_union_difference_L
+              !difference_diag_L !all_registers_union_l !difference_difference_L.
       f_equal. clear. set_solver. }
     { assert (12 + 65 = 77)%Z as ->;[done|]. rewrite Hscall_length in Hlink'. done. }
     iNext. iIntros "(HPC & Hr_stk & Hr_t0 & Hr_gen & Hstack_own & Hstack_adv & Hscall)".
     iDestruct (big_sepL2_length with "Hf2") as %Hf2_length. simpl in Hf2_length.
     assert (isCorrectPC_range pc_p pc_g pc_b pc_e s_last a_last) as Hvpc1.
-    { intros mid Hmid. assert (a0 <= s_last)%a as Hle;[apply contiguous_between_bounds in Hcont_scall; revert Hcont_scall Hcontge;clear; solve_addr|].
-      apply isCorrectPC_inrange with a0 a_last; auto.
+    { intros mid Hmid. assert (link0 <= s_last)%a as Hle;[apply contiguous_between_bounds in Hcont_scall; revert Hcont_scall Hcontge;clear; solve_addr|].
+      apply isCorrectPC_inrange with link0 a_last; auto.
       revert Hmid Hle. clear. solve_addr. }
-    (* jmp r_adv *)
-    iDestruct (big_sepL2_length with "Hf2") as %Hrest_length; simpl in Hrest_length. 
-    destruct rest0;[inversion Hrest_length|]. 
-    iPrologue rest0 Hrest_length "Hf2".
-    apply contiguous_between_cons_inv_first in Hcont_rest0 as Heq. subst a11. 
-    iApply (wp_jmp_success with "[$Hinstr $Hr_adv $HPC]");
-      [apply jmp_i|apply PermFlows_refl|iCorrectPC s_last a_last|..].
-    iEpilogue "(HPC & Hinstr & Hr_adv)". iSimpl in "HPC".
-    (* We now want to reason about unknown code. For this we invoke the fundamental theorem *)
+    
+    (* We now want to reason about unknown code. For this we invoke validity of wadv *)
     (* Before we can show the validity of the continuation, we need to set up the invariants 
        for local state, as well as the invariant for the stack *)
-    (* We start out by closing the invariant for the program *)
-    iMod ("Hcls" with "[Hprog_done Hinstr Hprog $Hna Hscall]") as "Hna". 
-    { iNext. iDestruct "Hprog_done" as "(Hpush3 & Hpush2 & Hpush1 & Ha_first)".
-      iFrame "Ha_first". rewrite Hrest_app. 
-      iApply (big_sepL2_app with "Hpush1 [-]"). 
-      iApply (big_sepL2_app with "Hpush2 [-]").
-      iApply (big_sepL2_app with "Hpush3 [-]").
-      iApply (big_sepL2_app with "Hscall [-]").
-      iFrame.
-    }
 
     (* We set the local stack frame and all the leftover Temporary resources to static *)
 
@@ -1805,19 +1856,19 @@ Section awkward_example.
     { apply contiguous_between_middle_bounds with (i:=3) (ai:=stack_own_b) in Hcont1;auto.
       revert Hcont1;clear. solve_addr. }
     iDestruct (region_mapsto_cons with "[Ha2 Hstack_own]") as "Hstack_own";[iContiguous_next Hcont1 1| |iFrame|].
-    { apply contiguous_between_middle_bounds with (i:=2) (ai:=a4) in Hcont1;auto.
+    { apply contiguous_between_middle_bounds with (i:=2) (ai:=a3) in Hcont1;auto.
       revert Hcont1;clear. solve_addr. }
     iDestruct (region_mapsto_cons with "[Hb_r Hstack_own]") as "Hstack_own";[iContiguous_next Hcont1 0| |iFrame|].
-    { apply contiguous_between_middle_bounds with (i:=1) (ai:=a3) in Hcont1;auto.
+    { apply contiguous_between_middle_bounds with (i:=1) (ai:=a2) in Hcont1;auto.
       revert Hcont1;clear. solve_addr. }
-
+    
     (* Next we want to define the map which will keep track of each word and permission *)
     iDestruct (temp_resources_split with "Hrest") as (pws) "[#Hrest_valid [#Hrev Hrest]]".
     iDestruct "Hrev" as %Hrev.
-    match goal with |- context [ [[a2,stack_own_last]]↦ₐ[RWLX][[ ?instrs ]]%I ] =>
+    match goal with |- context [ [[a0,stack_own_last]]↦ₐ[RWLX][[ ?instrs ]]%I ] =>
                     set l_frame := instrs
     end.
-    set m_static1 := lists_to_static_region_perms (region_addrs a2 stack_own_last ++ l')
+    set m_static1 := lists_to_static_region_perms (region_addrs a0 stack_own_last ++ l')
                                                   ((zip (repeat RWLX (length l_frame)) l_frame) ++ pws).
 
     (* we'll need that later to reason on the fact that the [zip] in the definition of
@@ -1825,9 +1876,9 @@ Section awkward_example.
     iDestruct (big_sepL2_length with "Hstack_own") as %Hlength_stack_own1.
 
     (* Allocate the static region containing the local stack frame and leftovers *)
-    assert (NoDup (region_addrs a2 stack_own_last ++ l')) as Hdup1.
+    assert (NoDup (region_addrs a0 stack_own_last ++ l')) as Hdup1.
     { rewrite Permutation_app_comm.
-      rewrite Hstack_eq in Hdup. apply region_addrs_of_contiguous_between in Hcont1.
+      rewrite Hstack_eq1 in Hdup. apply region_addrs_of_contiguous_between in Hcont1.
       rewrite Hcont1 app_assoc in Hdup. by apply NoDup_app in Hdup as [Hdup _]. }
     iDestruct (region_revoked_to_static (W.1, (<[i:=encode false]> W.2.1, W.2.2)) m_static1
                  with "[Hsts Hr Hstack_own Hrest]") as ">[Hsts Hr]".
@@ -1835,8 +1886,8 @@ Section awkward_example.
       iApply (big_sepL2_to_static_region_perms _ _ (λ a p w, a ↦ₐ[p] w)%I with "[] [Hstack_own Hrest]").
       - auto. 
       - iAlways.
-        iIntros (k y [p wy] Hin1 Hin2) "Hy /=".
-        iExists p,wy.
+        iIntros (k y [p' wy] Hin1 Hin2) "Hy /=".
+        iExists p',wy.
         destruct (decide (k < length (l_frame))). 
         + rewrite lookup_app_l in Hin1;[|rewrite Hlength_stack_own1;auto].
           rewrite lookup_app_l in Hin2;[|auto].
@@ -1846,10 +1897,11 @@ Section awkward_example.
           { apply zip_repeat_lookup_l with (b0:=RWLX) in l0 as [wy' Ha]. rewrite Hin2.
             rewrite Hin2 in Ha. inversion Ha. auto. }
           rewrite Hp in Hin2. inversion Hin2; subst.
-          repeat iSplit;auto. rewrite Hstack_eq. 
-          iDestruct (big_sepL_app with "Hstack_val") as "[Hframe _]".
+          repeat iSplit;auto. rewrite Hstack_eq1. 
+          iDestruct (big_sepL_app with "Hstack_region") as "[Hframe _]".
           apply region_addrs_of_contiguous_between in Hcont1. rewrite Hcont1.
-          iDestruct (big_sepL_lookup with "Hframe") as "Htest";[apply Hin1|auto].
+          iDestruct (big_sepL_and with "Hframe") as "[Htest _]". rewrite /read_write_cond. 
+          iDestruct (big_sepL_lookup with "Htest") as "Htest'";[apply Hin1|auto].
         + assert (length l_frame <= k);[revert n;clear;lia|]. 
           rewrite lookup_app_r in Hin1;[|rewrite Hlength_stack_own1;auto].
           rewrite lookup_app_r in Hin2;[|auto].
@@ -1866,20 +1918,23 @@ Section awkward_example.
     iDestruct (big_sepL2_length with "Hrest_valid") as %Hlength_rest. 
     iMod (monotone_close _ (region_addrs stack_own_last e_r) RWLX (λ Wv, interp Wv.1 Wv.2)
             with "[$Hsts $Hr Hstack_adv]") as "[Hsts Hr]".
-    { rewrite Hstack_eq. iDestruct (big_sepL_app with "Hstack_val") as "[_ Hstack_val']".
+    { rewrite Hstack_eq1. iDestruct (big_sepL_app with "Hstack_region") as "[_ Hstack_val']".
       iApply big_sepL_sep. iSplitL.
       - iDestruct (region_addrs_zeroes_trans with "Hstack_adv") as "Hstack_adv".
         iApply (big_sepL_mono with "Hstack_adv"). iIntros (k y Hsome) "Hy".
         iExists (inl 0%Z). iSplitR;auto. iFrame. simpl. iSplit.
         + iAlways. iIntros (W1 W2 Hrelated12) "HW1 /=". by repeat (rewrite fixpoint_interp1_eq /=).
         + by repeat (rewrite fixpoint_interp1_eq /=).
-      - iApply big_sepL_sep; iFrame "#". iApply big_sepL_forall. iPureIntro.
-        rewrite Hstack_eq in Hrevoked. apply Forall_app in Hrevoked as [_ Hrevoked]. 
+      - iDestruct (big_sepL_and with "Hstack_region") as "[Hstack_rel Hstack_pwl]".
+        rewrite /read_write_cond.
+         iDestruct (big_sepL_app with "Hstack_rel") as "[_ Hstack_rel']".
+         iApply big_sepL_sep; iFrame "#". iApply big_sepL_forall. iPureIntro.
+        rewrite Hstack_eq1 in Hrevoked. apply Forall_app in Hrevoked as [_ Hrevoked]. 
         intros k x Hsome.
-        assert (x ∉ (region_addrs a2 stack_own_last) ++ l') as Hnin.
+        assert (x ∉ (region_addrs a0 stack_own_last) ++ l') as Hnin.
         { apply elem_of_list_lookup_2 in Hsome.
           apply region_addrs_of_contiguous_between in Hcont1. 
-          rewrite Hstack_eq Hcont1 app_assoc in Hdup.
+          rewrite Hstack_eq1 Hcont1 app_assoc in Hdup.
           revert Hdup. rewrite Permutation_app_comm =>Hdup. apply NoDup_app in Hdup as [_ [Hnin _] ].
           apply Hnin in Hsome. rewrite Permutation_app_comm. auto. 
         }
@@ -1904,7 +1959,7 @@ Section awkward_example.
       intros x Hin. revert Hin. rewrite elements_list_to_set; auto. intros Hin.
       apply elem_of_app in Hin as [Hin | Hin].
       - revert Hrevoked. rewrite HeqW' Forall_forall =>Hrevoked. apply Hrevoked.
-        apply region_addrs_of_contiguous_between in Hcont1. rewrite Hstack_eq Hcont1. apply elem_of_app; by left.
+        apply region_addrs_of_contiguous_between in Hcont1. rewrite Hstack_eq1 Hcont1. apply elem_of_app; by left.
       - revert Hrev. rewrite Forall_forall =>Hrev. apply Hrev. auto.       
     }
     assert (related_sts_priv_world W W'') as HWW''.
@@ -1912,30 +1967,64 @@ Section awkward_example.
       eapply related_sts_priv_trans_world;[apply Hrelated|].
       auto. 
     }
+
     (* We choose the r *)
     set r : gmap RegName Word :=
       <[PC     := inl 0%Z]>
       (<[r_stk := inr (RWLX, Local, stack_own_last, e_r, stack_own_end)]>
-      (<[r_t0  := inr (E, Local, a2, e_r, stack_own_b)]>
-      (<[r_adv := inr (E, Global, b, e, a)]>
-      (create_gmap_default (list_difference all_registers [PC;r_stk;r_t0;r_adv]) (inl 0%Z))))).
+      (<[r_t0  := inr (E, Local, a0, e_r, stack_own_b)]>
+      (<[r_adv := inr (p, Global, b, e, a')]>
+       (create_gmap_default (list_difference all_registers [PC;r_stk;r_t0;r_adv]) (inl 0%Z))))).
+
+    (* Now that the world has been set up, we want to apply the jmp or fail patter of wadv *)
+    iDestruct (jmp_or_fail_spec _ _ φ with "Hadv_val") as "Hadv_cont". 
+    
+    (* jmp r_adv *)
+    iDestruct (big_sepL2_length with "Hf2") as %Hrest_length; simpl in Hrest_length. 
+    destruct rest0;[inversion Hrest0_length|]. 
+    iPrologue rest1 Hrest_length "Hf2".
+    apply contiguous_between_cons_inv_first in Hcont_rest1 as Heq. subst a11. 
+    iApply (wp_jmp_success with "[$Hinstr $Hr_adv $HPC]");
+      [apply jmp_i|apply PermFlows_refl|iCorrectPC s_last a_last|..].
+    (* before applying the eplogue, we want to distinguish between a correct or incorrect resulting PC *)
+    destruct (decide (isCorrectPC (updatePcPerm (inr (p, Global, b, e, a')))));
+      [rewrite decide_True;auto|rewrite decide_False;auto]. 
+    2: { iEpilogue "(HPC & _ & _)". iApply ("Hadv_cont" with "[Hφ $HPC]").
+         iApply "Hφ". iIntros (Hcontr). done. }
+    iDestruct "Hadv_cont" as (p0 g b0 e0 a11 Heq) "Hadv_cont". symmetry in Heq. simplify_eq.
+    iDestruct ("Hadv_cont" $! r _ HWW'') as "Hadv_contW''". 
+    iEpilogue "(HPC & Hinstr & Hr_adv)". iSimpl in "HPC".
+    
+    (* We close the invariant for the program *)
+    iMod ("Hcls" with "[Hprog_done Hinstr Hprog $Hna Hscall Hreqglob Hprestack]") as "Hna". 
+    { iNext. iDestruct "Hprog_done" as "(Hpush3 & Hpush2 & Hpush1 & Ha_first)".
+      rewrite Heqapp. 
+      iApply (big_sepL2_app with "Hreqglob [-]").
+      iApply (big_sepL2_app with "Hprestack [-]").
+      iFrame "Ha_first". rewrite Hrest_app. 
+      iApply (big_sepL2_app with "Hpush1 [-]"). 
+      iApply (big_sepL2_app with "Hpush2 [-]").
+      iApply (big_sepL2_app with "Hpush3 [-]").
+      iApply (big_sepL2_app with "Hscall [-]").
+      iFrame.
+    }
+    
     (* We have all the resources of r *)
-    iAssert (registers_mapsto (<[PC:=inr (RX, Global, b, e, a)]> r))
+    iAssert (registers_mapsto (<[PC:= (match p with
+                | E => inr (RX, Global, b, e, a')
+                | _ => inr (p, Global, b, e, a')
+                end)]> r))
       with "[Hr_gen Hr_stk Hr_t0 Hr_adv HPC]" as "Hmaps".
-    { iApply (registers_mapsto_resources with "Hr_gen Hr_stk Hr_t0 Hr_adv HPC").
-      rewrite !dom_delete_L dom_insert_L dom_insert_L Hrmap_dom.
+    { iApply (registers_mapsto_resources with "Hr_gen Hr_stk Hr_t0 Hr_adv HPC"). 
+      rewrite !dom_delete_L !dom_insert_L !dom_delete_L Hrmap_dom.
       rewrite !singleton_union_difference_L !all_registers_union_l !difference_difference_L.
       f_equal. clear. set_solver. }
     (* r contrains all registers *)
     iAssert (full_map r) as "#full";[iApply r_full|].
     iSimpl in "Hadv_val".
-    iAssert (interp_expression r W'' (inr (RX, Global, b, e, a)))
-      as "Hvalid". 
-    { iApply fundamental. iLeft; auto. iExists RX. iSplit;[iPureIntro;apply PermFlows_refl|]. 
-      iApply (adv_monotone with "Hadv_val"); auto. }
     (* We are now ready to show that all registers point to a valid word *)
     iAssert (∀ r1 : RegName, ⌜r1 ≠ PC⌝ → (fixpoint interp1) W'' (r !r! r1))%I
-      with "[-Hsts Hr Hmaps Hvalid Hna Hφ]" as "Hreg".
+      with "[-Hsts Hr Hmaps Hna Hφ]" as "Hreg".
     { iIntros (r1).
       assert (r1 = PC ∨ r1 = r_stk ∨ r1 = r_t0 ∨ r1 = r_adv ∨ (r1 ≠ PC ∧ r1 ≠ r_stk ∧ r1 ≠ r_t0 ∧ r1 ≠ r_adv)) as
           [-> | [-> | [-> | [Hr_t30 | [Hnpc [Hnr_stk [Hnr_t0 Hnr_t30] ] ] ] ] ] ].
@@ -1946,28 +2035,28 @@ Section awkward_example.
       }
       - iIntros "%". contradiction.
       - assert (r !! r_stk = Some (inr (RWLX, Local, stack_own_last, e_r, stack_own_end))) as Hr_stk; auto. 
-        rewrite /RegLocate Hr_stk fixpoint_interp1_eq. 
+        rewrite /RegLocate Hr_stk !fixpoint_interp1_eq. 
         iIntros (_). iExists RWLX. iSplitR; [auto|].
         iAssert ([∗ list] a ∈ region_addrs stack_own_last e_r, read_write_cond a RWLX (fixpoint interp1)
                              ∧ ⌜region_state_pwl W'' a⌝)%I as "#Hstack_adv_val". 
-        { rewrite Hstack_eq. 
-          iDestruct (big_sepL_app with "Hstack_val") as "[_ Hstack_val']".
+        { rewrite Hstack_eq1. 
+          iDestruct (big_sepL_app with "Hstack_region") as "[_ Hstack_val']".
           iApply (big_sepL_mono with "Hstack_val'").
-          iIntros (k y Hsome) "Hy".
-          rewrite Hstack_eq in Hrevoked.
+          iIntros (k y Hsome) "[Hy _]".
+          rewrite Hstack_eq1 in Hrevoked.
           apply Forall_app in Hrevoked as [_ Hrevoked].
           iFrame. iPureIntro. 
           apply close_list_std_sta_revoked.
           +  apply elem_of_list_lookup; eauto.
           + revert Hrevoked. rewrite Forall_forall =>Hrevoked.
-            assert (y ∉ (region_addrs a2 stack_own_last) ++ l') as Hnin.
+            assert (y ∉ (region_addrs a0 stack_own_last) ++ l') as Hnin.
             { apply elem_of_list_lookup_2 in Hsome.
               apply region_addrs_of_contiguous_between in Hcont1. 
-              rewrite Hstack_eq Hcont1 app_assoc in Hdup.
+              rewrite Hstack_eq1 Hcont1 app_assoc in Hdup.
                 revert Hdup. rewrite Permutation_app_comm =>Hdup. apply NoDup_app in Hdup as [_ [Hnin _] ].
                 apply Hnin in Hsome. rewrite Permutation_app_comm. auto. 
             }
-            rewrite std_sta_update_multiple_lookup_same_i /std /=. rewrite HeqW' in Hrevoked. 
+            rewrite std_sta_update_multiple_lookup_same_i /std /=. 
             apply Hrevoked. apply elem_of_list_lookup. eauto.
             rewrite lists_to_static_perms_region_dom.
             rewrite elements_list_to_set;auto. repeat rewrite app_length. auto. 
@@ -1978,12 +2067,12 @@ Section awkward_example.
         iIntros (y r' W3 Hay Hrelated3). iNext.
         iApply fundamental.
         + iRight. iRight. done.
-        + iExists RWLX. iSplit; auto. simpl.
+        + iExists RWLX. iSplit; auto. 
           iApply (adv_stack_monotone with "Hstack_adv_val"); auto. 
       - (* continuation *)
         iIntros (_).
-        assert (r !! r_t0 = Some (inr (E, Local, a2, e_r, stack_own_b))) as Hr_t0; auto. 
-        rewrite /RegLocate Hr_t0 fixpoint_interp1_eq. iSimpl. 
+        assert (r !! r_t0 = Some (inr (E, Local, a0, e_r, stack_own_b))) as Hr_t0; auto. 
+        rewrite /RegLocate Hr_t0 !fixpoint_interp1_eq. iSimpl. 
         (* prove continuation *)
         iAlways.
         iIntros (r' W3 Hrelated3).
@@ -1994,24 +2083,24 @@ Section awkward_example.
                  ⌜W3.1 !! a = Some Temporary⌝
                     ∗ rel a RWLX (λ Wv : WORLD * Word, ((fixpoint interp1) Wv.1) Wv.2)
                 )%I as "#Hstack_adv_tmp".
-        { rewrite Hstack_eq.
-          iDestruct (big_sepL_app with "Hstack_val") as "[_ Hstack_adv]".
-          iApply (big_sepL_mono with "Hstack_adv"). iIntros (k y Hsome) "Hr".
+        { rewrite Hstack_eq1.
+          iDestruct (big_sepL_app with "Hstack_region") as "[_ Hstack_adv]".
+          iApply (big_sepL_mono with "Hstack_adv"). iIntros (k y Hsome) "[Hr _]".
           rewrite /read_write_cond. iFrame. iPureIntro.
           assert (region_state_pwl W3 y) as Hlookup;[|auto].
-          revert Hrevoked; rewrite HeqW' Forall_forall =>Hrevoked.
+          revert Hrevoked; rewrite Forall_forall =>Hrevoked.
           apply region_state_pwl_monotone with W''; eauto.
           rewrite /W'' /region_state_pwl /std /=.
           apply close_list_std_sta_revoked; [apply elem_of_list_lookup; eauto|].
-          assert (y ∉ (region_addrs a2 stack_own_last) ++ l') as Hnin.
+          assert (y ∉ (region_addrs a0 stack_own_last) ++ l') as Hnin.
           { apply elem_of_list_lookup_2 in Hsome.
             apply region_addrs_of_contiguous_between in Hcont1. 
-            rewrite Hstack_eq Hcont1 app_assoc in Hdup.
+            rewrite Hstack_eq1 Hcont1 app_assoc in Hdup.
             revert Hdup. rewrite Permutation_app_comm =>Hdup. apply NoDup_app in Hdup as [_ [Hnin _] ].
             apply Hnin in Hsome. rewrite Permutation_app_comm. auto. 
           }
           rewrite std_sta_update_multiple_lookup_same_i /std /=. 
-          apply Hrevoked. rewrite Hstack_eq. apply elem_of_app; right. apply elem_of_list_lookup. eauto.
+          apply Hrevoked. rewrite Hstack_eq1. apply elem_of_app; right. apply elem_of_list_lookup. eauto.
           rewrite lists_to_static_perms_region_dom.
           rewrite elements_list_to_set;auto. repeat rewrite app_length. auto. 
         }
@@ -2020,20 +2109,20 @@ Section awkward_example.
         
         (* we want to distinguish between the case where the local stack frame is Static (step through 
            continuation) and where the local stack frame is temporary (apply FTLR) *)
-        assert (forall a, a ∈ region_addrs a2 stack_own_last ++ l' ->
+        assert (forall a, a ∈ region_addrs a0 stack_own_last ++ l' ->
                   (std W3) !! a = Some Temporary ∨
                   (std W3) !! a = Some (Static m_static1))
           as Hcases.
-        { intros a' Hin. apply or_comm,related_sts_pub_world_static with W'';auto.
+        { intros a'' Hin. apply or_comm,related_sts_pub_world_static with W'';auto.
           assert (std (std_update_multiple (revoke (W.1, (<[i:=encode false]> W.2.1, W.2.2)))
-                                           (elements (dom (gset Addr) m_static1)) (Static m_static1)) !! a' =
+                                           (elements (dom (gset Addr) m_static1)) (Static m_static1)) !! a'' =
                   Some (Static m_static1)) as Hlookup.
           { apply std_sta_update_multiple_lookup_in_i.
             rewrite lists_to_static_perms_region_dom;[|repeat rewrite app_length;rewrite Hlength_rest;auto].
             rewrite elements_list_to_set;auto. }
           rewrite -close_list_std_sta_same_alt;auto. rewrite Hlookup. intros Hcontr;inversion Hcontr as [heq].
         }
-        assert (a2 ∈ region_addrs a2 stack_own_last ++ l') as Ha2in.
+        assert (a0 ∈ region_addrs a0 stack_own_last ++ l') as Ha2in.
         { apply elem_of_app. left. apply elem_of_list_lookup. exists 0.
           apply region_addrs_of_contiguous_between in Hcont1 as <-. auto. }
         apply Hcases in Ha2in as [Hm_temp | Hm_static].
@@ -2046,26 +2135,26 @@ Section awkward_example.
                If it is temp we are done. If it is static then we can use the full_sts_static_all lemma 
                to assert that a2 is also in state Static, which leads to a contradiction, as we are in the 
                case where it should be Temporary *)
-            iIntros (a'). rewrite /m_static1. 
+            iIntros (a''). rewrite /m_static1. 
             rewrite lists_to_static_perms_region_dom;[|repeat rewrite app_length;rewrite Hlength_rest;auto].
             iIntros (Hin). apply elem_of_list_to_set in Hin. 
-            pose proof (Hcases a' Hin) as [Htemp' | Hstatic].
+            pose proof (Hcases a'' Hin) as [Htemp' | Hstatic].
             - rewrite /temporary. rewrite Htemp'. auto.
             - iDestruct (full_sts_static_all with "Hsts Hr") as %Hforall;[eauto|]. exfalso.
-              assert (a2 ∈ dom (gset Addr) m_static1) as Hin'.
+              assert (a0 ∈ dom (gset Addr) m_static1) as Hin'.
               { rewrite lists_to_static_perms_region_dom;[|repeat rewrite app_length;rewrite Hlength_rest;auto].
                 apply elem_of_list_to_set. apply elem_of_app. left. apply elem_of_list_lookup. exists 0.
                 apply region_addrs_of_contiguous_between in Hcont1 as <-. auto. }
               apply Hforall in Hin'. rewrite /static Hm_temp in Hin'. done. 
           }
-          iDestruct (fundamental W3 r' RX Local a2 e_r stack_own_b with "[] [] [-]") as "[_ Hcont]";[by iLeft| |iFrame "∗ #"|..].
+          iDestruct (fundamental W3 r' RX Local a0 e_r stack_own_b with "[] [] [-]") as "[_ Hcont]";[by iLeft| |iFrame "∗ #"|..].
           { iSimpl. iExists RWLX. iSplit;[auto|].
-            iApply (big_sepL_mono with "Hstack_val").
-            iIntros (k y Hk) "Hrel". iFrame. iPureIntro.            
+            iApply (big_sepL_mono with "Hstack_region").
+            iIntros (k y Hk) "[Hrel _]". iFrame. iPureIntro.            
             left.
             (* we assert that the region is all in state temporary *)
             rewrite (region_addrs_split _ stack_own_last) in Hk. 
-            assert (y ∈ region_addrs a2 stack_own_last ++ region_addrs stack_own_last e_r) as Hk'.
+            assert (y ∈ region_addrs a0 stack_own_last ++ region_addrs stack_own_last e_r) as Hk'.
             { apply elem_of_list_lookup. eauto. }
             apply elem_of_app in Hk' as [Hframe | Hadv].
             + assert (y ∈ dom (gset Addr) m_static1) as Hk'.
@@ -2122,10 +2211,10 @@ Section awkward_example.
         iDestruct (region_static_to_revoked with "[$Hr $Hsts]") as ">(Hsts & Hr & Hm_static1_resources & _)". eauto.
 
         (* finally we split up the static resources into the local stack frame and l' *)
-        iAssert ([[a2,stack_own_last]] ↦ₐ[RWLX] [[l_frame]]
+        iAssert ([[a0,stack_own_last]] ↦ₐ[RWLX] [[l_frame]]
                 ∗ [∗ list] a;pw ∈ l';pws, a ↦ₐ[pw.1] pw.2)%I with "[Hm_static1_resources]" as "[Hframe Hl']".
         { rewrite /m_static1 /region_mapsto /static_resources.
-          iAssert (([∗ list] y1;y2 ∈ region_addrs a2 stack_own_last;zip (repeat RWLX (length l_frame)) l_frame, y1 ↦ₐ[y2.1] y2.2)
+          iAssert (([∗ list] y1;y2 ∈ region_addrs a0 stack_own_last;zip (repeat RWLX (length l_frame)) l_frame, y1 ↦ₐ[y2.1] y2.2)
                      ∗ ([∗ list] a11;pw ∈ l';pws, a11 ↦ₐ[pw.1] pw.2))%I with "[-]" as "[H $]".
           { iApply (big_sepL2_app' _ _ _ (λ k a pv, a ↦ₐ[pv.1] pv.2))%I;auto.
             iApply (static_region_perms_to_big_sepL2 _ _ (λ a p w, a ↦ₐ[p] w) with "[] Hm_static1_resources")%I. 
@@ -2137,9 +2226,9 @@ Section awkward_example.
 
         (* we isolate the activation record from the frame *)
         iDestruct (region_mapsto_cons with "Hframe") as "[Ha2 Hframe]"; [iContiguous_next Hcont1 0|..].
-        { apply contiguous_between_middle_bounds with (i:=1) (ai:=a3) in Hcont1;auto. revert Hcont1;clear;solve_addr. }
+        { apply contiguous_between_middle_bounds with (i:=1) (ai:=a2) in Hcont1;auto. revert Hcont1;clear;solve_addr. }
         iDestruct (region_mapsto_cons with "Hframe") as "[Ha3 Hframe]"; [iContiguous_next Hcont1 1|..].
-        { apply contiguous_between_middle_bounds with (i:=2) (ai:=a4) in Hcont1;auto. revert Hcont1;clear;solve_addr. }
+        { apply contiguous_between_middle_bounds with (i:=2) (ai:=a3) in Hcont1;auto. revert Hcont1;clear;solve_addr. }
         iDestruct (region_mapsto_cons with "Hframe") as "[Ha4 Hframe]"; [iContiguous_next Hcont1 2|..].
         { apply contiguous_between_middle_bounds with (i:=3) (ai:=stack_own_b) in Hcont1;auto.
           revert Hcont1;clear;solve_addr. }
@@ -2150,70 +2239,73 @@ Section awkward_example.
           exists a. solve_addr. }
 
         (* step through instructions in activation record *)
+        destruct rest1;[by inversion Hrest_length|].
         iApply (scall_epilogue_spec with "[-]"); last iFrame "Hframe HPC";
-          [|done|iContiguous_next Hcont_rest0 0|apply Hstack_new|revert Hstack_own_bound Hstack_own_bound'; clear; solve_addr|..].
+          [|done|iContiguous_next Hcont_rest1 0|apply Hstack_new|revert Hstack_own_bound Hstack_own_bound'; clear; solve_addr|..].
         { intros mid Hmid. split;[|auto]. apply withinBounds_le_addr in Hwb2.
           apply (contiguous_between_middle_bounds _ 3 stack_own_b) in Hcont1;[|auto]. revert Hwb2 Hcont1 Hmid. clear. solve_addr.
         }
         iSplitL "Hr_t1";[iNext;eauto|]. iSplitL "Hr_stk";[iNext;eauto|]. 
         iNext. iIntros "(HPC & Hr_stk & Hr_t1 & Hframe)".
         iDestruct "Hr_t1" as (wrt1) "Hr_t1".
-
+        
         (* we can now step through the rest of the program *)
         (* to do that wee need to open the non atomic invariant of the program *)
         iMod (na_inv_open with "Hf4 Hna") as "(>Hprog & Hna & Hcls')";[solve_ndisj..|]. 
-        rewrite Hrest_app /=. repeat rewrite app_comm_cons. 
-        iDestruct (mapsto_decomposition _ _ _ (take 84 (awkward_instrs r_adv 65)) with "Hprog")
+        rewrite Heqapp Hrest_app. repeat rewrite app_assoc. repeat rewrite app_comm_cons. rewrite app_assoc.
+
+        iDestruct (mapsto_decomposition _ _ _ (take 122 (awkward_instrs r_adv 65)) with "Hprog")
           as "[Hprog_done [Ha Hprog] ]". 
-        { simpl. inversion Hscall_length as [Heq]. rewrite Heq. omega. }
+        { simpl. repeat rewrite app_length /=.
+          rewrite Hscall_length Hprepstack_length Hreqglob_length. auto. }
         (* let's prove some practical lemmas before continuing *)
         (* assert (last (rest0_first :: a9 :: rest0) = Some a_last) as Hlast0. *)
         (* { rewrite Hrest_app in Hlast. repeat rewrite app_comm_cons in Hlast. *)
         (*   by rewrite -last_app_eq in Hlast; [|simpl;lia]. } *)
         iCombine "Ha" "Hprog_done" as "Hprog_done".
         (* sub r_t1 0 7 *)
-        iPrologue rest0 Hrest_length "Hprog".
+        iPrologue rest1 Hrest_length "Hprog".
         iApply (wp_add_sub_lt_success_z_z with "[$HPC $Hr_t1 $Hinstr]");
-          [apply sub_z_z_i|right;left;eauto|iContiguous_next Hcont_rest0 1|apply PermFlows_refl|iCorrectPC s_last a_last|..]. 
+          [apply sub_z_z_i|right;left;eauto|iContiguous_next Hcont_rest1 1|apply PermFlows_refl|iCorrectPC s_last a_last|..]. 
         iEpilogue "(HPC & Hinstr & Hr_t1)".
         iCombine "Hinstr" "Hprog_done" as "Hprog_done".
         (* lea r_stk r_t1 *)
-        iPrologue rest0 Hrest_length "Hprog". 
-        assert ((stack_new + (0 - 7))%a = Some a4) as Hpop.
-        { assert ((a4 + 1)%a = Some stack_own_b) as Ha0;[iContiguous_next Hcont1 2|].
+        iPrologue rest1 Hrest_length "Hprog". 
+        assert ((stack_new + (0 - 7))%a = Some a3) as Hpop.
+        { assert ((a3 + 1)%a = Some stack_own_b) as Ha0;[iContiguous_next Hcont1 2|].
           revert Ha0 Hstack_own_bound' Hstack_new. clear. solve_addr. }
         iApply (wp_lea_success_reg with "[$HPC $Hr_t1 $Hr_stk $Hinstr]");
-          [apply lea_r_i|apply PermFlows_refl|iCorrectPC s_last a_last|iContiguous_next Hcont_rest0 2|apply Hpop|auto..].
+          [apply lea_r_i|apply PermFlows_refl|iCorrectPC s_last a_last|iContiguous_next Hcont_rest1 2|apply Hpop|auto..].
         iEpilogue "(HPC & Hinstr & Hr_t1 & Hr_stk)". iCombine "Hinstr" "Hprog_done" as "Hprog_done". 
         (* pop r_stk r_adv *)
-        do 3 (destruct rest0; [inversion Hrest_length|]).
-        iDestruct (big_sepL2_app_inv _ [a13;a14;a15] (a16::rest0) with "Hprog") as "[Hpop Hprog]";[simpl;auto|].
-        clear Hpop. assert ((a4 + (0 - 1))%a = Some a3) as Hpop.
-        { rewrite -(addr_add_assoc a3 _ 1);[apply addr_add_0|iContiguous_next Hcont1 1]. }
+        do 3 (destruct rest1; [inversion Hrest_length|]).
+        iDestruct (big_sepL2_app_inv _ [a13;a14;a15] (a16::rest1) with "Hprog") as "[Hpop Hprog]";[simpl;auto|].
+        clear Hpop. assert ((a3 + (0 - 1))%a = Some a2) as Hpop.
+        { rewrite -(addr_add_assoc a2 _ 1);[apply addr_add_0|iContiguous_next Hcont1 1]. }
         iApply (pop_spec); [..|iFrame "HPC Hr_stk Hr_t1 Hpop Hr_adv Ha4"];
-          [split;[|split];iCorrectPC s_last a_last| apply PermFlows_refl|iContiguous_bounds_withinBounds a2 stack_own_last|auto|
-           iContiguous_next Hcont_rest0 3|iContiguous_next Hcont_rest0 4|iContiguous_next Hcont_rest0 5|apply Hpop|].
+          [split;[|split];iCorrectPC s_last a_last| apply PermFlows_refl|iContiguous_bounds_withinBounds a0 stack_own_last|auto|
+           iContiguous_next Hcont_rest1 3|iContiguous_next Hcont_rest1 4|iContiguous_next Hcont_rest1 5|apply Hpop|].
         iNext. iIntros "(HPC & Hpop & Hr_adv & Ha4 & Hr_stk & Hr_t1)". iCombine "Hpop" "Hprog_done" as "Hprog_done".
         (* pop r_stk r_self *)
-        do 3 (destruct rest0; [inversion Hrest_length|]).
-        iDestruct (big_sepL2_app_inv _ [a16;a17;a18] (a19::rest0) with "Hprog") as "[Hpop Hprog]";[simpl;auto|].
-        clear Hpop. assert ((a3 + (0 - 1))%a = Some a2) as Hpop.
-        { rewrite -(addr_add_assoc a2 _ 1);[apply addr_add_0|iContiguous_next Hcont1 0]. }
+        do 3 (destruct rest1; [inversion Hrest_length|]).
+        iDestruct (big_sepL2_app_inv _ [a16;a17;a18] (a19::rest1) with "Hprog") as "[Hpop Hprog]";[simpl;auto|].
+        clear Hpop. assert ((a2 + (0 - 1))%a = Some a0) as Hpop.
+        { rewrite -(addr_add_assoc a0 _ 1);[apply addr_add_0|iContiguous_next Hcont1 0]. }
         iApply (pop_spec); [..|iFrame "HPC Hr_stk Hr_t1 Hpop Hr_t0 Ha3"];
-          [split;[|split];iCorrectPC s_last a_last| apply PermFlows_refl|iContiguous_bounds_withinBounds a2 stack_own_last|auto|
-           iContiguous_next Hcont_rest0 6|iContiguous_next Hcont_rest0 7|iContiguous_next Hcont_rest0 8|apply Hpop|].
+          [split;[|split];iCorrectPC s_last a_last| apply PermFlows_refl|iContiguous_bounds_withinBounds a0 stack_own_last|auto|
+           iContiguous_next Hcont_rest1 6|iContiguous_next Hcont_rest1 7|iContiguous_next Hcont_rest1 8|apply Hpop|].
         iNext. iIntros "(HPC & Hpop & Hr_t0 & Ha3 & Hr_stk & Hr_t1)". iCombine "Hpop" "Hprog_done" as "Hprog_done".
         (* pop r_stk r_env *)
-        do 3 (destruct rest0; [inversion Hrest_length|]).
-        iDestruct (big_sepL2_app_inv _ [a19;a20;a21] (a22::rest0) with "Hprog") as "[Hpop Hprog]";[simpl;auto|].
-        clear Hpop. assert ((a2 + (0 - 1))%a = Some b_r') as Hpop.
+        do 3 (destruct rest1; [inversion Hrest_length|]).
+        iDestruct (big_sepL2_app_inv _ [a19;a20;a21] (a22::rest1) with "Hprog") as "[Hpop Hprog]";[simpl;auto|].
+        clear Hpop. assert ((a0 + (0 - 1))%a = Some b_r') as Hpop.
         { rewrite -(addr_add_assoc b_r' _ 1);[apply addr_add_0|auto]. }
         iApply (pop_spec); [..|iFrame "HPC Hr_stk Hr_t1 Hpop Hr_env Ha2"];
-          [split;[|split];iCorrectPC s_last a_last| apply PermFlows_refl|iContiguous_bounds_withinBounds a2 stack_own_last|auto|
-           iContiguous_next Hcont_rest0 9|iContiguous_next Hcont_rest0 10|iContiguous_next Hcont_rest0 11|apply Hpop|].
+          [split;[|split];iCorrectPC s_last a_last| apply PermFlows_refl|iContiguous_bounds_withinBounds a0 stack_own_last|auto|
+           iContiguous_next Hcont_rest1 9|iContiguous_next Hcont_rest1 10|iContiguous_next Hcont_rest1 11|apply Hpop|].
         iNext. iIntros "(HPC & Hpop & Hr_env & Hb_r & Hr_stk & Hr_t1)". iCombine "Hpop" "Hprog_done" as "Hprog_done".
         (* store r_env 1 *)
-        iPrologue rest0 Hrest_length "Hprog".
+        iPrologue rest1 Hrest_length "Hprog".
         (* Storing 1 will always constitute a public future world of 
            std_update_multiple (revoke W3) dom(m_static1) Revoked *)
         iAssert (∀ φ, ▷ (PC ↦ᵣ inr (pc_p, pc_g, pc_b, pc_e, a23)
@@ -2236,7 +2328,7 @@ Section awkward_example.
           destruct y; iDestruct "Hb" as ">Hb".
           - iApply (wp_store_success_z with "[$HPC $Hinstr $Hr_env $Hb]");
               [apply store_z_i|apply PermFlows_refl|apply PermFlows_refl|iCorrectPC s_last a_last|
-               iContiguous_next Hcont_rest0 12|auto|].
+               iContiguous_next Hcont_rest1 12|auto|].
             iNext. iIntros "(HPC & Hinstr & Hr_env & Hd)".
             iMod ("Hcls" with "[Hstate Hd]") as "_".
             { iNext. iExists true. iFrame. }
@@ -2246,9 +2338,9 @@ Section awkward_example.
             eauto. 
           - iApply (wp_store_success_z with "[$HPC $Hinstr $Hr_env $Hb]");
               [apply store_z_i|apply PermFlows_refl|apply PermFlows_refl|iCorrectPC s_last a_last|
-               iContiguous_next Hcont_rest0 12|auto|].
+               iContiguous_next Hcont_rest1 12|auto|].
             iNext. iIntros "(HPC & Hinstr & Hr_env & Hd)".
-            iMod (sts_update_loc _ _ _ true with "Hsts Hstate") as "[Hsts Hstate] /=".
+            iMod (sts_update_loc _ _ _ true with "Hsts Hstate") as "[Hsts Hstate]".
             iMod ("Hcls" with "[Hstate Hd]") as "_".
             { iNext. iExists true. iFrame. }
             iModIntro. iApply wp_pure_step_later;auto;iNext. iApply "Hφ".
@@ -2264,17 +2356,17 @@ Section awkward_example.
         iDestruct "HW3lookup" as %[HW3lookup Hw3rel]. 
         iCombine "Hinstr" "Hprog_done" as "Hprog_done".
         (* push r_stk r_env *)
-        do 2 (destruct rest0;[inversion Hrest_length|]).
-        iDestruct (big_sepL2_app_inv _ [a23;a24] (a25::rest0) with "Hprog") as "[Hpush Hprog]";[simpl;auto|]. 
+        do 2 (destruct rest1;[inversion Hrest_length|]).
+        iDestruct (big_sepL2_app_inv _ [a23;a24] (a25::rest1) with "Hprog") as "[Hpush Hprog]";[simpl;auto|]. 
         iApply (push_r_spec);[..|iFrame "HPC Hr_stk Hpush Hr_env Hb_r"];
-          [split;iCorrectPC s_last a_last|apply PermFlows_refl|auto|iContiguous_next Hcont_rest0 13|iContiguous_next Hcont_rest0 14|auto|..].
+          [split;iCorrectPC s_last a_last|apply PermFlows_refl|auto|iContiguous_next Hcont_rest1 13|iContiguous_next Hcont_rest1 14|auto|..].
         iNext. iIntros "(HPC & Hpush & Hr_stk & Hr_env & Hb_r)". iCombine "Hpush" "Hprog_done" as "Hprog_done".
         (* push r_stk r_self *)
-        do 2 (destruct rest0;[inversion Hrest_length|]).
-        iDestruct (big_sepL2_app_inv _ [a25;a26] (a27::rest0) with "Hprog") as "[Hpush Hprog]";[simpl;auto|]. 
+        do 2 (destruct rest1;[inversion Hrest_length|]).
+        iDestruct (big_sepL2_app_inv _ [a25;a26] (a27::rest1) with "Hprog") as "[Hpush Hprog]";[simpl;auto|]. 
         iApply (push_r_spec);[..|iFrame "HPC Hr_stk Hpush Hr_t0 Ha3"];
-          [split;iCorrectPC s_last a_last|apply PermFlows_refl|iContiguous_bounds_withinBounds a2 stack_own_last|iContiguous_next Hcont_rest0 15|
-           iContiguous_next Hcont_rest0 16|iContiguous_next Hcont1 0|..].
+          [split;iCorrectPC s_last a_last|apply PermFlows_refl|iContiguous_bounds_withinBounds a0 stack_own_last|iContiguous_next Hcont_rest1 15|
+           iContiguous_next Hcont_rest1 16|iContiguous_next Hcont1 0|..].
         iNext. iIntros "(HPC & Hpush & Hr_stk & Hr_self & Ha3)". iCombine "Hpush" "Hprog_done" as "Hprog_done". 
         (* SECOND SCALL *)
 
@@ -2302,47 +2394,47 @@ Section awkward_example.
         iAssert (∃ ws_adv : list Word, [[stack_own_end,e_r]]↦ₐ[RWLX][[ws_adv]])%I with "[Hstack_adv Hlast']" as (ws_adv'') "Hstack_adv".
         { iDestruct (region_addrs_exists with "Hstack_adv") as (ws_adv') "Hstack_adv".
           iDestruct (big_sepL2_sep with "Hstack_adv") as "[_ Hstack_adv]". iDestruct (big_sepL2_sep with "Hstack_adv") as "[Hstack_adv _]".
-          iDestruct (mapsto_decomposition _ _ _ [inr (RWLX, Local, a2, e_r, stack_own_end)] with "[$Hstack_adv $Hlast']") as "Hstack_adv";[auto|..].
+          iDestruct (mapsto_decomposition _ _ _ [inr (RWLX, Local, a0, e_r, stack_own_end)] with "[$Hstack_adv $Hlast']") as "Hstack_adv";[auto|..].
           rewrite Hstack_localeq. 
           iExists (_ :: ws_adv'). iFrame. 
         }
-        iAssert (∃ ws_own : list Word, [[a4,stack_own_end]]↦ₐ[RWLX][[ws_own]])%I with "[Hframe Ha4]" as (ws_own'') "Hstack_own".
-        { iExists ((inr (E, Global, b, e, a)) :: _). rewrite /region_mapsto.
-          assert ([a4] ++ region_addrs stack_own_b stack_own_end = region_addrs a4 stack_own_end) as <-.
+        iAssert (∃ ws_own : list Word, [[a3,stack_own_end]]↦ₐ[RWLX][[ws_own]])%I with "[Hframe Ha4]" as (ws_own'') "Hstack_own".
+        { iExists ((inr (p, Global, b, e, a')) :: _). rewrite /region_mapsto.
+          assert ([a3] ++ region_addrs stack_own_b stack_own_end = region_addrs a3 stack_own_end) as <-.
           { rewrite /region_addrs.
-            assert ((a4 + 1)%a = Some stack_own_b) as Hincr;[iContiguous_next Hcont1 2|].
-            assert (region_size a4 stack_own_end = S (region_size stack_own_b stack_own_end)) as ->.
+            assert ((a3 + 1)%a = Some stack_own_b) as Hincr;[iContiguous_next Hcont1 2|].
+            assert (region_size a3 stack_own_end = S (region_size stack_own_b stack_own_end)) as ->.
             { revert Hstack_own_bound' Hincr; clear. rewrite /region_size. solve_addr. }
             simpl. f_equiv. rewrite Hincr /=. done. 
           }
-          iApply (mapsto_decomposition [a4] _ _ [inr (E, Global, b, e, a)]); [auto|]. iFrame. done.
+          iApply (mapsto_decomposition [a3] _ _ [inr (p, Global, b, e, a')]); [auto|]. iFrame. done.
         }
         (* prepare for scall *)
         (* split the program into the scall_prologue and the rest *)
-        assert (contiguous_between (a27 :: rest0) a27 a_last) as Hcont_weak.
-        { repeat (inversion Hcont_rest0 as [|????? Hf2']; subst; auto; clear Hcont_rest0; rename Hf2' into Hcont_rest0). }
-        iDestruct (contiguous_between_program_split with "Hprog") as (scall_prologue1 rest1 s_last1)
+        assert (contiguous_between (a27 :: rest1) a27 a_last) as Hcont_weak.
+        { repeat (inversion Hcont_rest1 as [|????? Hcont_rest1']; subst; auto; clear Hcont_rest1; rename Hcont_rest1' into Hcont_rest1). }
+        iDestruct (contiguous_between_program_split with "Hprog") as (scall_prologue1 rest2 s_last1)
                                                                        "(Hscall & Hprog & #Hcont)"; [eauto|..].
         clear Hcont_weak.
-        iDestruct "Hcont" as %(Hcont_scall1 & Hcont_rest1 & Hrest_app1 & Hlink1). subst.
+        iDestruct "Hcont" as %(Hcont_scall1 & Hcont_rest2 & Hrest_app1 & Hlink2). subst.
         iDestruct (big_sepL2_length with "Hscall") as %Hscall_length1. simpl in Hscall_length1.
         destruct scall_prologue1 as [|scall_prologue_first1 scall_prologue1];[inversion Hscall_length1|].
         assert (scall_prologue_first1 = a27) as <-;[inversion Hrest_app1;auto|].
         (* some important element of the stack *)
-        assert ((a4 + 8)%a = Some stack_own_end) as Hstack_own_bound1.
-        { assert ((a4 + 1)%a = Some stack_own_b) as Ha4;[iContiguous_next Hcont1 2|].
+        assert ((a3 + 8)%a = Some stack_own_end) as Hstack_own_bound1.
+        { assert ((a3 + 1)%a = Some stack_own_b) as Ha4;[iContiguous_next Hcont1 2|].
           revert Hstack_own_bound Hstack_own_bound' Ha4. clear. solve_addr. }
-        assert ((a4 + 7)%a = Some stack_new) as Hstack_own_bound1'.
+        assert ((a3 + 7)%a = Some stack_new) as Hstack_own_bound1'.
         { revert Hstack_own_bound1 Hstack_new. clear. solve_addr. }
         assert (scall_prologue_first1 < s_last1)%a as Hcontlt1.
-        { revert Hscall_length1 Hlink1. clear. solve_addr. }
+        { revert Hscall_length1 Hlink2. clear. solve_addr. }
         assert (s_last <= scall_prologue_first1)%a as Hcontge1.
-        { apply region_addrs_of_contiguous_between in Hcont_scall. subst. revert Hscall_length1 Hcont_rest0 Hcontlt1.  clear =>Hscall_length Hf2 Hcontlt.
+        { apply region_addrs_of_contiguous_between in Hcont_scall. subst. revert Hscall_length1 Hcont_rest1 Hcontlt1.  clear =>Hscall_length Hf2 Hcontlt.
           apply contiguous_between_middle_bounds with (i := 17) (ai := scall_prologue_first1) in Hf2;[solve_addr|auto]. 
         }
-        assert (withinBounds (RWLX, Local, a2, e_r, stack_own_end) = true) as Hwb3.
+        assert (withinBounds (RWLX, Local, a0, e_r, stack_own_end) = true) as Hwb3.
         { isWithinBounds. 
-          - assert ((a2 + 3)%a = Some stack_own_b) as Hincr;[apply contiguous_between_incr_addr with (i := 3) (ai := stack_own_b) in Hcont1; auto|].
+          - assert ((a0 + 3)%a = Some stack_own_b) as Hincr;[apply contiguous_between_incr_addr with (i := 3) (ai := stack_own_b) in Hcont1; auto|].
             revert Hstack_own_bound' Hincr. clear. solve_addr. 
           - apply withinBounds_le_addr in Hwb2 as [_ Hwb2]. revert Hstack_own_bound Hstack_own_bound' Hwb2. clear. solve_addr. 
         }
@@ -2364,52 +2456,31 @@ Section awkward_example.
           [| |apply Hwb3|apply Hcont_scall1|apply PermFlows_refl|
            iNotElemOfList| |iContiguous_next Hcont1 1|apply Hstack_own_bound1'|apply Hstack_own_bound1|
            | done |..].
-        { assert (s_last1 <= a_last)%a as Hle;[by apply contiguous_between_bounds in Hcont_rest1|].
-          intros mid Hmid. apply isCorrectPC_inrange with a0 a_last; auto.
+        { assert (s_last1 <= a_last)%a as Hle;[by apply contiguous_between_bounds in Hcont_rest2|].
+          intros mid Hmid. apply isCorrectPC_inrange with link0 a_last; auto.
           revert Hle Hcontlt1 Hcontge1 Hcontlt Hcontge Hmid. clear; intros. split; solve_addr. }
-        { iContiguous_bounds_withinBounds a2 stack_own_last. }
+        { iContiguous_bounds_withinBounds a0 stack_own_last. }
         { repeat rewrite ?dom_insert_L ?dom_delete_L. rewrite Hdom_r'.
           rewrite !singleton_union_difference_L !all_registers_union_l !difference_difference_L.
           f_equal. clear. set_solver. }
-        { assert (12 + 65 = 77)%Z as ->;[done|]. rewrite Hscall_length1 in Hlink1. done. }
+        { assert (12 + 65 = 77)%Z as ->;[done|]. rewrite Hscall_length1 in Hlink2. done. }
         iNext. iIntros "(HPC & Hr_stk & Hr_t0 & Hr_gen & Hstack_own & Hstack_adv & Hscall)".
         iDestruct (big_sepL2_length with "Hprog") as %Hrest_length1. simpl in Hrest_length1.
         assert (isCorrectPC_range pc_p pc_g pc_b pc_e s_last1 a_last) as Hvpc2.
-        { intros mid Hmid. assert (a0 <= s_last1)%a as Hle.
+        { intros mid Hmid. assert (link0 <= s_last1)%a as Hle.
           { apply contiguous_between_bounds in Hcont_scall1.
             apply contiguous_between_bounds in Hcont_scall.
             revert Hcont_scall Hcont_scall1 Hcontge1 Hcontge;clear. solve_addr.
           } 
-          apply isCorrectPC_inrange with a0 a_last; auto.
+          apply isCorrectPC_inrange with link0 a_last; auto.
           revert Hmid Hle. clear. solve_addr. }
         (* jmp r_adv *)
-        destruct rest1;[inversion Hrest_length1|]. 
-        iPrologue rest1 Hrest_length1 "Hprog". apply contiguous_between_cons_inv_first in Hcont_rest1 as Heq. subst s_last1. 
-        iApply (wp_jmp_success with "[$Hinstr $Hr_adv $HPC]");
-          [apply jmp_i|apply PermFlows_refl|iCorrectPC a27 a_last|..].
-        iEpilogue "(HPC & Hinstr & Hr_adv)". iSimpl in "HPC".
-        (* again we are jumping to unknown code. We will now need to close all our invariants so we can 
-           reestablish the FTLR on the new state *)
-        (* we close the invariant for our program *)
-        iMod ("Hcls'" with "[Hprog_done Hprog Hinstr Hscall $Hna]") as "Hna".
-        { iNext. iDestruct "Hprog_done" as "(Hpush2 & push1 & Ha19 & Hpop1 & Hpop2 & Hpop3 &
-                                             Ha8 & Ha9 & Hrest0_first & Hprog_done)".
-          iApply (big_sepL2_app with "Hprog_done [-]").
-          iFrame "Hrest0_first Ha9 Ha8". 
-          iApply (big_sepL2_app with "Hpop3 [-]").
-          iApply (big_sepL2_app with "Hpop2 [-]").
-          iApply (big_sepL2_app with "Hpop1 [-]").
-          iFrame "Ha19".
-          iApply (big_sepL2_app with "push1 [-]").
-          iApply (big_sepL2_app with "Hpush2 [-]").
-          rewrite Hrest_app1. 
-          iApply (big_sepL2_app with "Hscall [-]"). iFrame.
-        }
-
+        destruct rest2;[inversion Hrest_length1|]. 
+        iPrologue rest2 Hrest_length1 "Hprog". apply contiguous_between_cons_inv_first in Hcont_rest2 as Heq. subst s_last1. 
         (* we separate the points to chunk from the persistent parts of the leftovers l'' *)
         iDestruct (temp_resources_split with "Hrest'") as (pws') "[#Hrest_valid' [#Hrev Hrest']]".
         iDestruct "Hrev" as %Hrev'.
-
+        
         (* Allocate a static region to hold our frame *)
 
         (* first, put together again the resources for the frame *)
@@ -2419,7 +2490,7 @@ Section awkward_example.
         { revert Hstack_own_bound1. clear; solve_addr. }
         iDestruct (region_mapsto_cons with "[$Hb_r $Hstack_own]") as "Hstack_own";
           [iContiguous_next Hcont1 0|..].
-        { have: (a3 + 1 = Some a4)%a. by iContiguous_next Hcont1 1. revert Hstack_own_bound1.
+        { have: (a2 + 1 = Some a3)%a. by iContiguous_next Hcont1 1. revert Hstack_own_bound1.
           clear; solve_addr. }
 
         (* we'll need that later to reason on the fact that the [zip] in the definition of
@@ -2427,10 +2498,10 @@ Section awkward_example.
         iDestruct (big_sepL2_length with "Hstack_own") as %Hlength_stack_own2.
         iDestruct (big_sepL2_length with "Hrest'") as %Hlength_rest''.
 
-        match goal with |- context [ [[a2,stack_own_end]]↦ₐ[RWLX][[ ?instrs ]]%I ] =>
+        match goal with |- context [ [[a0,stack_own_end]]↦ₐ[RWLX][[ ?instrs ]]%I ] =>
           set l_frame2 := instrs
         end.
-        set static2_addrs := region_addrs a2 stack_own_end ++ l' ++ l''.
+        set static2_addrs := region_addrs a0 stack_own_end ++ l' ++ l''.
         set static2_instrs := (zip (repeat RWLX (length l_frame2)) l_frame2) ++ pws ++ pws'.
         set m_static2 := lists_to_static_region_perms static2_addrs static2_instrs.
 
@@ -2450,49 +2521,51 @@ Section awkward_example.
 
         iAssert ([∗ list] a;pw ∈ l';pws, static_res a pw.1 pw.2)%I with "[Hl']" as "Hl'".
         { iDestruct (big_sepL2_sep with "[Hrest_valid $Hl']") as "Hl'". by iApply "Hrest_valid".
-          iApply (big_sepL2_mono with "Hl'"). cbn. iIntros (k a' pw ? ?) "[H1 H2]".
+          iApply (big_sepL2_mono with "Hl'"). cbn. iIntros (k a'' pw ? ?) "[H1 H2]".
           iDestruct "H2" as (? ? ?) "(? & ? & ?)". iExists _. iFrame. eauto. }
-
+        
         iAssert ([∗ list] a;pw ∈ l'';pws', static_res a pw.1 pw.2)%I with "[Hrest']" as "Hrest'".
         { iDestruct (big_sepL2_sep with "[Hrest_valid' $Hrest']") as "Hrest'". by iApply "Hrest_valid'".
-          iApply (big_sepL2_mono with "Hrest'"). cbn. iIntros (k a' pw ? ?) "[H1 H2]".
+          iApply (big_sepL2_mono with "Hrest'"). cbn. iIntros (k a'' pw ? ?) "[H1 H2]".
           iDestruct "H2" as (? ? ?) "(? & ? & ?)". iExists _. iFrame. eauto. }
 
-        assert (a2 <= stack_own_end ∧ stack_own_end <= e_r)%a.
+        assert (a0 <= stack_own_end ∧ stack_own_end <= e_r)%a.
         { move: (withinBounds_le_addr _ _ _ _ _ Hwb3). clear; solve_addr. }
 
-        iAssert ([∗ list] a;w ∈ (region_addrs a2 stack_own_end);l_frame2, static_res a RWLX w)%I
+        iAssert ([∗ list] a;w ∈ (region_addrs a0 stack_own_end);l_frame2, static_res a RWLX w)%I
           with "[Hstack_own]" as "Hstack_own".
-        { rewrite (region_addrs_split a2 stack_own_end e_r) //.
-          iDestruct (big_sepL_app with "Hstack_val") as "[Hstack_val' _]".
+        { rewrite (region_addrs_split a0 stack_own_end e_r) //.
+          iDestruct (big_sepL_app with "Hstack_region") as "[Hstack_val' _]".
           iDestruct (big_sepL2_sep with "[Hstack_val' $Hstack_own]") as "Hstack_own".
           { iApply big_sepL2_to_big_sepL_l. auto. iApply "Hstack_val'". }
-          iApply (big_sepL2_mono with "Hstack_own"). iIntros (? ? ? ? ?) "(? & ?)". unfold static_res.
-          iExists _. iFrame. iSplitR; [iPureIntro; congruence|]. iPureIntro. intro; apply interp_persistent. }
+          iApply (big_sepL2_mono with "Hstack_own"). iIntros (? ? ? ? ?) "(? & ? & ?)". unfold static_res.
+          iExists _. rewrite /read_write_cond. iFrame. iSplitR; [iPureIntro; congruence|]. iPureIntro.
+          intro; apply interp_persistent. }
 
         iDestruct (big_sepL2_app with "Hl' Hrest'") as "Hl'_rest'".
 
         (* we will need that later *)
-        iAssert (⌜NoDup (region_addrs a2 e_r ++ l' ++ l'')⌝)%I as %Hstack_l'_l''_NoDup.
+        iAssert (⌜NoDup (region_addrs a0 e_r ++ l' ++ l'')⌝)%I as %Hstack_l'_l''_NoDup.
         { iAssert ([∗ list] a;w ∈ (region_addrs stack_own_end e_r);region_addrs_zeroes stack_own_end e_r, static_res a RWLX w)%I
             with "[Hstack_adv]" as "Hstack_adv".
-          { rewrite (region_addrs_split a2 stack_own_end e_r) //.
-            iDestruct (big_sepL_app with "Hstack_val") as "[_ Hstack_val']".
+          { rewrite (region_addrs_split a0 stack_own_end e_r) //.
+            iDestruct (big_sepL_app with "Hstack_region") as "[_ Hstack_val']".
             iDestruct (big_sepL2_sep with "[Hstack_val' $Hstack_adv]") as "Hstack_adv".
             { iApply big_sepL2_to_big_sepL_l.
               (* TODO: region_addrs_length, region_addrs_zeroes_length *)
               by rewrite /region_addrs !region_addrs_aux_length /region_addrs_zeroes repeat_length //.
               iApply "Hstack_val'". }
-            iApply (big_sepL2_mono with "Hstack_adv"). iIntros (? ? ? ? ?) "(? & ?)". unfold static_res.
-            iExists _. iFrame. iSplitR; [iPureIntro; congruence|]. iPureIntro. intro; apply interp_persistent. }
-
+            iApply (big_sepL2_mono with "Hstack_adv"). iIntros (? ? ? ? ?) "(? & ? & ?)". unfold static_res.
+            unfold read_write_cond. iExists _. iFrame. iSplitR; [iPureIntro; congruence|].
+            iPureIntro. intro; apply interp_persistent. }
+          
           iApply (NoDup_of_sepL2_exclusive with "[] [Hstack_own Hstack_adv Hl'_rest']").
-          2: { rewrite (region_addrs_split a2 stack_own_end e_r) //.
+          2: { rewrite (region_addrs_split a0 stack_own_end e_r) //.
                iDestruct (big_sepL2_app with "Hstack_own Hstack_adv") as "Hstack".
                iDestruct (big_sepL2_zip_repeat with "Hstack") as "Hstack".
                iDestruct (big_sepL2_app with "Hstack Hl'_rest'") as "HH". iApply "HH". }
           iIntros (? [? ?] [? ?]). iApply Hstatic_res_excl. }
-
+        
         (* Allocate the static region; for that we only need the part of Hstack we own *)
         iAssert ([∗ list] a;pw ∈ static2_addrs;static2_instrs, static_res a pw.1 pw.2)%I
           with "[Hstack_own Hl'_rest']" as "Hstatic".
@@ -2511,18 +2584,18 @@ Section awkward_example.
         rewrite -std_update_multiple_revoke_commute;auto.
 
         (* now that we have privately updated our resources, we can close the region invariant for the adv stack *)
-        assert (list.last (a2 :: a3 :: a4 :: stack_own_b :: stack_own) = Some stack_own_end) as Hlast.
-        { apply contiguous_between_link_last with a2 stack_own_last; [auto|apply gt_Sn_O|].
+        assert (list.last (a0 :: a2 :: a3 :: stack_own_b :: stack_own) = Some stack_own_end) as Hlast.
+        { apply contiguous_between_link_last with a0 stack_own_last; [auto|apply gt_Sn_O|].
           revert Hstack_own_bound Hstack_own_bound'; clear. solve_addr. }
 
         (* To make some of the future proofs easier, let's make certain assertions about addresses in adv frame *)
         assert (∀ a, a ∈ region_addrs stack_own_end e_r -> a ∉ elements (dom (gset Addr) m_static2)) as Hnin2.
         { rewrite lists_to_static_perms_region_dom.
           2: { repeat rewrite app_length. rewrite Hlength_rest Hlength_rest''. auto. }
-          intros a' Ha'. 
+          intros a'' Ha'. 
           rewrite elements_list_to_set;auto.
-          assert (a' ∈ region_addrs a2 e_r) as Hin'.
-          { rewrite -Hstack_localeq in Ha'. rewrite Hstack_eq.
+          assert (a'' ∈ region_addrs a0 e_r) as Hin'.
+          { rewrite -Hstack_localeq in Ha'. rewrite Hstack_eq1.
             apply elem_of_app in Ha' as [Hl | Hr].
             - apply elem_of_list_singleton in Hl. subst.
               apply elem_of_app; left. apply elem_of_list_lookup. exists (11 - 1).
@@ -2537,10 +2610,10 @@ Section awkward_example.
         assert (∀ a, a ∈ region_addrs stack_own_last e_r -> a ∉ elements (dom (gset Addr) m_static1)) as Hnin1.
         { rewrite lists_to_static_perms_region_dom.
           2: { repeat rewrite app_length. rewrite Hlength_rest . auto. }
-          intros a' Ha'. 
+          intros a'' Ha'. 
           rewrite elements_list_to_set;auto.
-          assert (a' ∈ region_addrs a2 e_r) as Hin'.
-          { rewrite Hstack_eq. apply elem_of_app;right. auto. } 
+          assert (a'' ∈ region_addrs a0 e_r) as Hin'.
+          { rewrite Hstack_eq1. apply elem_of_app;right. auto. } 
           apply not_elem_of_app. split.
           - apply region_addrs_xor_elem_of with (c:=stack_own_last) in Hin' as [ [Hin' Hnin] | [Hin' Hnin] ];auto.
             eapply withinBounds_le_addr. apply Hwb2.
@@ -2572,23 +2645,24 @@ Section awkward_example.
         iMod (monotone_close _ (region_addrs stack_own_end e_r) RWLX (λ Wv, interp Wv.1 Wv.2)
                 with "[$Hsts $Hr Hstack_adv ]") as "[Hsts Hr]".
         { iClear "Hreg' Hfull' full Hf4 Hrel Hinv Hadv_val".
-          rewrite Hstack_eq. 
+          rewrite Hstack_eq1. 
           iDestruct (region_addrs_zeroes_trans with "Hstack_adv") as "Hstack_adv".
           rewrite /region_mapsto -Hstack_localeq.
           iDestruct (big_sepL_app with "Hstack_adv") as "[ [Hs_last' _] Hstack_adv]". 
-          iDestruct (big_sepL_app with "Hstack_val") as "[Hstack_last Hstack_val']".
-          iDestruct (big_sepL_lookup _ _ (length (a2 :: a3 :: a4 :: stack_own_b :: stack_own) - 1) stack_own_end with "Hstack_last") as "Hs_last_val";[by rewrite -last_lookup|].
+          iDestruct (big_sepL_app with "Hstack_region") as "[Hstack_last Hstack_val']".
+          iDestruct (big_sepL_lookup _ _ (length (a0 :: a2 :: a3 :: stack_own_b :: stack_own) - 1) stack_own_end with "Hstack_last") as "[Hs_last_val _]";[by rewrite -last_lookup|].
           iApply big_sepL_sep. iSplitL.
           - iApply big_sepL_app. iSplitL "Hs_last'". 
-            + iSimpl. iSplit;[|auto]. iExists (inl 0%Z). iSplitR;auto. iFrame. simpl. iSplit.
-              * iAlways. iIntros (W1 W2 Hrelated12) "HW1 /=". by repeat (rewrite fixpoint_interp1_eq /=).
-              * by repeat (rewrite fixpoint_interp1_eq /=).
+            + iSimpl. iSplit;[|auto]. iExists (inl 0%Z). iSplitR;auto. iFrame. iSplit.
+              * iAlways. iIntros (W1 W2 Hrelated12) "HW1". by repeat (rewrite fixpoint_interp1_eq).
+              * by repeat (rewrite fixpoint_interp1_eq).
             + iApply (big_sepL_mono with "Hstack_adv"). iIntros (k y Hsome) "Hy".
-              iExists (inl 0%Z). iSplitR;auto. iFrame. simpl. iSplit.
-              * iAlways. iIntros (W1 W2 Hrelated12) "HW1 /=". by repeat (rewrite fixpoint_interp1_eq /=).
-              * by repeat (rewrite fixpoint_interp1_eq /=).
-          - iApply big_sepL_sep; iFrame "#". iSplit;[auto|]. iApply big_sepL_forall. iPureIntro.
-            hnf. intros x a' Hin.
+              iExists (inl 0%Z). iSplitR;auto. iFrame. iSplit.
+              * iAlways. iIntros (W1 W2 Hrelated12) "HW1". by repeat (rewrite fixpoint_interp1_eq).
+              * by repeat (rewrite fixpoint_interp1_eq).
+          - iDestruct (big_sepL_and with "Hstack_val'") as "[Hstack_rel _]". 
+            iApply big_sepL_sep; iFrame "#". iSplit;[auto|]. iApply big_sepL_forall. iPureIntro.
+            hnf. intros x a'' Hin.
             apply Hlookup_revoked. apply elem_of_list_lookup. eauto. 
         }
 
@@ -2603,12 +2677,12 @@ Section awkward_example.
           eapply related_sts_priv_trans_world;[|apply revoke_related_sts_priv];auto.
           apply related_sts_pub_priv_world. destruct HW3lookup as [y Hy].
           split;[apply related_sts_std_pub_refl|simpl;eapply related_pub_local_1; eauto].
-          - apply Forall_forall. intros a' Hin.
+          - apply Forall_forall. intros a'' Hin.
             apply revoke_lookup_Static. apply elem_of_elements in Hin. 
             apply Hall_static in Hin. rewrite /static in Hin.
-            destruct (W3.1 !! a') eqn:Hsome;[subst|done]; auto.
-          - apply Forall_forall. intros a' Hin.
-            destruct (decide (a' ∈ (elements (dom (gset Addr) m_static1)))). 
+            destruct (W3.1 !! a'') eqn:Hsome;[subst|done]; auto.
+          - apply Forall_forall. intros a'' Hin.
+            destruct (decide (a'' ∈ (elements (dom (gset Addr) m_static1)))). 
             apply std_sta_update_multiple_lookup_in_i;auto.
             rewrite std_sta_update_multiple_lookup_same_i;auto.
             apply revoke_lookup_Temp. apply Hiff'. revert Hin n.
@@ -2626,12 +2700,26 @@ Section awkward_example.
         set r2 : gmap RegName Word :=
           <[PC    := inl 0%Z]>
           (<[r_stk := inr (RWLX, Local, stack_own_end, e_r, stack_new)]>
-          (<[r_t0  := inr (E, Local, a2, e_r, a4)]>
-          (<[r_adv := inr (E, Global, b, e, a)]>
+          (<[r_t0  := inr (E, Local, a0, e_r, a3)]>
+          (<[r_adv := inr (p, Global, b, e, a')]>
           (create_gmap_default
              (list_difference all_registers [PC; r_stk; r_t0; r_adv]) (inl 0%Z))))).
+
+        (* we set up the expression relation of the jump *)
+        assert (related_sts_priv_world W W5) as Hrelated5'.
+        { eapply related_sts_priv_trans_world;[|apply Hrelated5]. 
+            by eapply related_sts_priv_pub_trans_world;[|apply Hrelated3]. }
+        iDestruct ("Hadv_cont" $! r2 W5 Hrelated5') as "Hadv_contW5".     
+        (* we do the actual jump *)
+        iApply (wp_jmp_success with "[$Hinstr $Hr_adv $HPC]");
+          [apply jmp_i|apply PermFlows_refl|iCorrectPC a27 a_last|..].
+        iEpilogue "(HPC & Hinstr & Hr_adv)". iSimpl in "HPC".
+
         (* We have all the resources of r *)
-        iAssert (registers_mapsto (<[PC:=inr (RX, Global, b, e, a)]> r2))
+        iAssert (registers_mapsto (<[PC:=match p with
+                | E => inr (RX, Global, b, e, a')
+                | _ => inr (p, Global, b, e, a')
+                end]> r2))
           with "[Hr_gen Hr_stk Hr_t0 Hr_adv HPC]" as "Hmaps".
         { iApply (registers_mapsto_resources with "Hr_gen Hr_stk Hr_t0 Hr_adv HPC").
           repeat rewrite ?dom_delete_L ?dom_insert_L. rewrite Hdom_r'.
@@ -2640,26 +2728,45 @@ Section awkward_example.
         (* r contrains all registers *)
         iAssert (full_map r2) as "#Hfull2";[iApply r_full|].
         iSimpl in "Hadv_val".
-        iAssert (interp_expression r2 W5 (inr (RX, Global, b, e, a)))
-          as "Hvalid". 
-        { iApply fundamental. iLeft; auto. iExists RX. iSplit;[iPureIntro;apply PermFlows_refl|]. 
-          iApply (adv_monotone with "Hadv_val"). 
-          eapply related_sts_priv_trans_world;[|apply Hrelated5].
-            by eapply related_sts_priv_pub_trans_world;[|apply Hrelated3]. }
+        (* again we are jumping to unknown code. We will now need to close all our invariants so we can 
+           reestablish the FTLR on the new state *)
+        (* we close the invariant for our program *)
+        iMod ("Hcls'" with "[Hprog_done Hprog Hinstr Hscall $Hna]") as "Hna".
+        { iNext. iDestruct "Hprog_done" as "(Hpush2 & push1 & Ha19 & Hpop1 & Hpop2 & Hpop3 &
+                                             Ha8 & Ha9 & Hrest0_first & Hprog_done)".
+          iApply (big_sepL2_app with "Hprog_done [-]"). 
+          iFrame "Hrest0_first Ha9 Ha8". 
+          iApply (big_sepL2_app with "Hpop3 [-]").
+          iApply (big_sepL2_app with "Hpop2 [-]").
+          iApply (big_sepL2_app with "Hpop1 [-]").
+          iFrame "Ha19".
+          iApply (big_sepL2_app with "push1 [-]").
+          iApply (big_sepL2_app with "Hpush2 [-]").
+          rewrite Hrest_app1. 
+          iApply (big_sepL2_app with "Hscall [-]"). iFrame.
+        }
+
+        
+        (* iAssert (interp_expression r2 W5 (inr (RX, Global, b, e, a))) *)
+        (*   as "Hvalid".  *)
+        (* { iApply fundamental. iLeft; auto. iExists RX. iSplit;[iPureIntro;apply PermFlows_refl|].  *)
+        (*   iApply (adv_monotone with "Hadv_val").  *)
+        (*   eapply related_sts_priv_trans_world;[|apply Hrelated5]. *)
+        (*     by eapply related_sts_priv_pub_trans_world;[|apply Hrelated3]. } *)
         (* the adversary stack is valid in the W5 *)
         iAssert ([∗ list] a ∈ region_addrs stack_own_end e_r,
                  read_write_cond a RWLX (fixpoint interp1)
                  ∗ ⌜region_state_pwl W5 a⌝)%I as "#Hstack_adv_val".
-        { rewrite Hstack_eq.
-          iDestruct (big_sepL_app with "Hstack_val") as "[Hstack_last Hstack_val']".
-          iDestruct (big_sepL_lookup _ _ (length (a2 :: a3 :: a4 :: stack_own_b :: stack_own) - 1) stack_own_end with "Hstack_last")
-            as "Hs_last_val";[by rewrite -last_lookup|].
+        { rewrite Hstack_eq1.
+          iDestruct (big_sepL_app with "Hstack_region") as "[Hstack_last Hstack_val']".
+          iDestruct (big_sepL_lookup _ _ (length (a0 :: a2 :: a3 :: stack_own_b :: stack_own) - 1) stack_own_end with "Hstack_last")
+            as "[Hs_last_val _]";[by rewrite -last_lookup|].
           iApply big_sepL_sep. iSplit.
           - rewrite /region_mapsto -Hstack_localeq. 
             iApply big_sepL_app. iFrame "Hs_last_val".
             iSplit;[auto|]. 
             iApply (big_sepL_mono with "Hstack_val'").
-            iIntros (g y Hsome) "Hy". iFrame.
+            iIntros (g y Hsome) "[Hy _]". rewrite /read_write_cond. iFrame.
           - iApply big_sepL_forall. iPureIntro.
             intros g y Hsome.
             apply close_list_std_sta_revoked; auto.
@@ -2669,7 +2776,7 @@ Section awkward_example.
         }
         (* We are now ready to show that all registers point to a valid word *)
         iAssert (∀ r1 : RegName, ⌜r1 ≠ PC⌝ → (fixpoint interp1) W5 (r2 !r! r1))%I
-          with "[-Hsts Hr Hmaps Hvalid Hna]" as "Hreg".
+          with "[-Hsts Hr Hmaps Hna]" as "Hreg".
         { iIntros (r1).
           assert (r1 = PC ∨ r1 = r_stk ∨ r1 = r_t0 ∨ r1 = r_adv ∨ (r1 ≠ PC ∧ r1 ≠ r_stk ∧ r1 ≠ r_t0 ∧ r1 ≠ r_adv)) as
               [-> | [-> | [-> | [Hr_t30 | [Hnpc [Hnr_stk [Hnr_t0 Hnr_t30] ] ] ] ] ] ].
@@ -2691,11 +2798,11 @@ Section awkward_example.
             iIntros (y r3 W6 Hay Hrelated6). iNext.
             iApply fundamental.
             + iRight. iRight. done.
-            + iExists RWLX. iSplit; auto. simpl.
+            + iExists RWLX. iSplit; auto. 
               iApply (adv_stack_monotone with "Hstack_adv_val'"); auto. 
           - (* continuation *)
             iIntros (_). clear Hr_t0. 
-            assert (r2 !! r_t0 = Some (inr (E, Local, a2, e_r, a4))) as Hr_t0; auto. 
+            assert (r2 !! r_t0 = Some (inr (E, Local, a0, e_r, a3))) as Hr_t0; auto. 
             rewrite /RegLocate Hr_t0. repeat rewrite fixpoint_interp1_eq. iSimpl. 
             (* prove continuation *)
             iAlways.
@@ -2716,21 +2823,21 @@ Section awkward_example.
             
             (* we want to distinguish between the case where the local stack frame is Static (step through 
                continuation) and where the local stack frame is temporary (apply FTLR) *)
-            assert (forall a, a ∈ region_addrs a2 stack_own_end ++ l' ++ l'' ->
+            assert (forall a, a ∈ region_addrs a0 stack_own_end ++ l' ++ l'' ->
                          (std W6) !! a = Some Temporary ∨
                          (std W6) !! a = Some (Static m_static2))
               as Hcases'.
-            { intros a' Hin. apply or_comm,related_sts_pub_world_static with W5;auto.
-              assert (std W4 !! a' = Some (Static m_static2)) as Hlookup.
+            { intros a'' Hin. apply or_comm,related_sts_pub_world_static with W5;auto.
+              assert (std W4 !! a'' = Some (Static m_static2)) as Hlookup.
                 { apply std_sta_update_multiple_lookup_in_i.
                   rewrite lists_to_static_perms_region_dom;[|repeat rewrite app_length;rewrite Hlength_rest;auto].
                   rewrite elements_list_to_set;auto. }
                 rewrite -close_list_std_sta_same_alt;auto. rewrite Hlookup. intros Hcontr;inversion Hcontr as [heq].
             }
-            assert (a2 ∈ region_addrs a2 stack_own_end ++ l' ++ l'') as Ha2in.
+            assert (a0 ∈ region_addrs a0 stack_own_end ++ l' ++ l'') as Ha2in.
             { apply elem_of_app. left. apply elem_of_list_lookup. exists 0.
-              apply region_addrs_first. assert ((a2 + 2)%a = Some a4) as Hincr.
-              eapply (contiguous_between_incr_addr _ 2 a2 a4);[apply Hcont1|auto].
+              apply region_addrs_first. assert ((a0 + 2)%a = Some a3) as Hincr.
+              eapply (contiguous_between_incr_addr _ 2 a0 a3);[apply Hcont1|auto].
               revert Hstack_own_bound1 Hincr. clear. solve_addr. }
             pose proof (Hcases' _ Ha2in) as [Hm_temp' | Hm_static'].
             { iSimpl. 
@@ -2738,25 +2845,25 @@ Section awkward_example.
               iSplit; [auto|rewrite /interp_conf].
               (* first we want to assert that if a2 is Temporary, the remaining addresses are also temporary *)
               iAssert (⌜∀ a : Addr, a ∈ dom (gset Addr) m_static2 → temporary W6 a⌝)%I as %Hm_frame_temp_all.
-              { iIntros (a'). rewrite /m_static2. 
+              { iIntros (a''). rewrite /m_static2. 
                 rewrite lists_to_static_perms_region_dom;[|repeat rewrite app_length;rewrite Hlength_rest;auto].
                 iIntros (Hin). apply elem_of_list_to_set in Hin. 
-                pose proof (Hcases' a' Hin) as [Htemp' | Hstatic].
+                pose proof (Hcases' a'' Hin) as [Htemp' | Hstatic].
                 - rewrite /temporary. rewrite Htemp'. auto.
                 - iDestruct (full_sts_static_all with "Hsts Hr") as %Hforall;[eauto|]. exfalso.
-                  assert (a2 ∈ dom (gset Addr) m_static2) as Hin'.
+                  assert (a0 ∈ dom (gset Addr) m_static2) as Hin'.
                   { rewrite lists_to_static_perms_region_dom;[|repeat rewrite app_length;rewrite Hlength_rest;auto].
                     apply elem_of_list_to_set. auto. }
                   apply Hforall in Hin'. rewrite /static Hm_temp' in Hin'. done. 
               }
-              iDestruct (fundamental W6 r3 RX Local a2 e_r a4 with "[] [] [-]") as "[_ Hcont]";[by iLeft| |iFrame "∗ #"|..].
+              iDestruct (fundamental W6 r3 RX Local a0 e_r a3 with "[] [] [-]") as "[_ Hcont]";[by iLeft| |iFrame "∗ #"|..].
               { iSimpl. iExists RWLX. iSplit;[auto|].
-                iApply (big_sepL_mono with "Hstack_val").
-                iIntros (k y Hk) "Hrel". iFrame. iPureIntro.            
+                iApply (big_sepL_mono with "Hstack_region").
+                iIntros (k y Hk) "[Hrel _]". iFrame. iPureIntro.            
                 left. 
                 (* we assert that the region is all in state temporary *)
                 rewrite (region_addrs_split _ stack_own_end) in Hk. 
-                assert (y ∈ region_addrs a2 stack_own_end ++ region_addrs stack_own_end e_r) as Hk'.
+                assert (y ∈ region_addrs a0 stack_own_end ++ region_addrs stack_own_end e_r) as Hk'.
                 { apply elem_of_list_lookup. eauto. }
                 apply elem_of_app in Hk' as [Hframe | Hadv].
                 + assert (y ∈ dom (gset Addr) m_static2) as Hk'.
@@ -2791,26 +2898,26 @@ Section awkward_example.
             (* Open the static region for the local stack frame *)
             iDestruct (region_open_static with "[$Hr $Hsts]") as "(Hr & Hsts & Hstates & Hframe & %)";
               [apply Hm_static'|].
-            iAssert ( a2 ↦ₐ[RWLX] inr (RWX, Global, d, d', d)
-                    ∗ a3 ↦ₐ[RWLX] inr (E, g_ret, b_ret, e_ret, a_ret)
-                    ∗ [[a4,stack_own_end]] ↦ₐ[RWLX] 
+            iAssert ( a0 ↦ₐ[RWLX] inr (RWX, Global, d, d', d)
+                    ∗ a2 ↦ₐ[RWLX] wret
+                    ∗ [[a3,stack_own_end]] ↦ₐ[RWLX] 
                            [[ [inl w_1; inl w_2; inl w_3; inl w_4a; inl w_4b; inl w_4c;
-                               inr (pc_p, pc_g, pc_b, pc_e, a27); inr (RWLX, Local, a2, e_r, stack_new)] ]]
+                               inr (pc_p, pc_g, pc_b, pc_e, a27); inr (RWLX, Local, a0, e_r, stack_new)] ]]
                     ∗ [∗ list] a;pw ∈ l'++l''; pws++pws', a ↦ₐ[pw.1] pw.2)%I
               with "[Hframe]" as "(Ha2 & Ha3 & Hframe & Hrest)".
             { iDestruct (static_region_perms_to_big_sepL2 _ _ (λ a p v, a ↦ₐ[p] v)%I with "[] Hframe")
                 as "Hframe";[auto|..]. 
               { repeat rewrite app_length. rewrite Hlength_rest Hlength_rest'';auto. }
               { iAlways. iIntros (k pw1 pw2 Hlookup1 Hlookup2) "Hr".
-                iDestruct "Hr" as (p v Heq) "Hr". inversion Heq. iFrame. 
+                iDestruct "Hr" as (p' v Heq) "Hr". inversion Heq. iFrame. 
               }
               iDestruct (big_sepL2_app' with "Hframe") as "[Hframe $]";[auto|].
               iDestruct (big_sepL2_zip_repeat _ _ (λ a p v, a ↦ₐ[p] v)%I with "Hframe") as "Hframe".
               iDestruct (region_mapsto_cons with "Hframe") as "[Ha2 Hframe]"; [iContiguous_next Hcont1 0|..].
-              { apply contiguous_between_middle_bounds with (i:=1) (ai:=a3) in Hcont1;auto.
+              { apply contiguous_between_middle_bounds with (i:=1) (ai:=a2) in Hcont1;auto.
                 revert Hstack_own_bound Hstack_own_bound' Hcont1;clear. solve_addr. }
               iDestruct (region_mapsto_cons with "Hframe") as "[Ha3 Hframe]"; [iContiguous_next Hcont1 1|..].
-              { apply contiguous_between_middle_bounds with (i:=2) (ai:=a4) in Hcont1;auto.
+              { apply contiguous_between_middle_bounds with (i:=2) (ai:=a3) in Hcont1;auto.
                 revert Hstack_own_bound Hstack_own_bound' Hcont1;clear. solve_addr. }
               iFrame. 
             }
@@ -2820,9 +2927,9 @@ Section awkward_example.
               exists a. solve_addr. }
             (* step through instructions in activation record *)
             iApply (scall_epilogue_spec with "[-]"); last iFrame "Hframe HPC";
-              [|done|iContiguous_next Hcont_rest1 0|apply Hstack_new_1|revert Hstack_own_bound1 Hstack_own_bound1'; clear; solve_addr|..].
+              [|done|iContiguous_next Hcont_rest2 0|apply Hstack_new_1|revert Hstack_own_bound1 Hstack_own_bound1'; clear; solve_addr|..].
             { intros mid Hmid. split;[|auto]. apply withinBounds_le_addr in Hwb3.
-              apply (contiguous_between_middle_bounds _ 2 a4) in Hcont1;[|auto].
+              apply (contiguous_between_middle_bounds _ 2 a3) in Hcont1;[|auto].
               revert Hwb3 Hcont1 Hmid. clear. solve_addr. 
             }
             iSplitL "Hr_t1";[iNext;eauto|]. iSplitL "Hr_stk";[iNext;eauto|]. 
@@ -2831,10 +2938,13 @@ Section awkward_example.
             (* we don't want to close the stack invariant yet, as we will now need to pop it *)
             (* go through rest of the program. We will now need to open the invariant and destruct it into its done and prog part *)
             (* sub r_t1 0 7 *)
-            iMod (na_inv_open with "Hf4 Hna") as "(>Hprog & Hna & Hcls')";[solve_ndisj..|]. 
-            rewrite Hrest_app1 /=. repeat rewrite app_comm_cons. rewrite app_assoc.
+            iMod (na_inv_open with "Hf4 Hna") as "(>Hprog & Hna & Hcls')";[solve_ndisj..|].
+            iClear "Hadv_val". 
+            rewrite Hrest_app1. repeat rewrite app_comm_cons. rewrite app_assoc.
             rewrite /awkward_example /awkward_instrs.
-            iDestruct (mapsto_decomposition _ _ _ ([store_z r_env 0] ++
+            iDestruct (mapsto_decomposition _ _ _ (reqglob_instrs r_adv ++
+                                                   prepstack_instrs r_stk 11 ++ 
+                                                   [store_z r_env 0] ++
                                                    push_r_instrs r_stk r_env ++
                                                    push_r_instrs r_stk r_t0 ++
                                                    push_r_instrs r_stk r_adv ++
@@ -2850,7 +2960,7 @@ Section awkward_example.
                                                    push_r_instrs r_stk r_t0 ++
                                                    scall_prologue_instrs 65 r_adv) with "Hprog")
               as "[Hprog_done [Ha Hprog] ]". 
-            { simpl. inversion Hscall_length as [Heq]. inversion Hscall_length1 as [Heq']. rewrite app_length Heq /=. rewrite Heq'. done. }
+            { simpl. inversion Hscall_length as [Heq]. inversion Hscall_length1 as [Heq']. rewrite app_length Heq /=. rewrite Heq'. repeat rewrite app_length. rewrite Hreqglob_length Hprepstack_length. simpl. repeat f_equiv. rewrite Heq. done. }
             (* let's prove some practical lemmas before continuing *)
             (* assert (last (rest1_first :: a27 :: rest1) = Some a_last) as Hlast1. *)
             (* { rewrite Hrest_app in Hlast. repeat rewrite app_comm_cons in Hlast. *)
@@ -2859,43 +2969,43 @@ Section awkward_example.
             (*   by rewrite -last_app_eq in Hlast;[|simpl;apply gt_Sn_O]. } *)
             iCombine "Ha" "Hprog_done" as "Hprog_done".
             (* sub r_t1 0 7 *)
-            iPrologue rest1 Hrest_length1 "Hprog".
+            iPrologue rest2 Hrest_length1 "Hprog".
             iApply (wp_add_sub_lt_success_z_z with "[$HPC Hr_t1 $Hinstr]");
-              [apply sub_z_z_i|right;left;eauto|iContiguous_next Hcont_rest1 1|apply PermFlows_refl|iCorrectPC a27 a_last|
+              [apply sub_z_z_i|right;left;eauto|iContiguous_next Hcont_rest2 1|apply PermFlows_refl|iCorrectPC a27 a_last|
                iSimpl;iFrame;eauto|].
             iEpilogue "(HPC & Hinstr & Hr_t1)".
             iCombine "Hinstr" "Hprog_done" as "Hprog_done".
             (* lea r_stk r_t1 *)
-            iPrologue rest1 Hrest_length1 "Hprog". 
-            assert ((stack_new_1 + (0 - 7))%a = Some a3) as Hpop1.
-            { assert ((a4 + 1)%a = Some stack_own_b) as Hincr;[iContiguous_next Hcont1 2|].
-              assert ((a3 + 1)%a = Some a4) as Hincr';[iContiguous_next Hcont1 1|].
+            iPrologue rest2 Hrest_length1 "Hprog". 
+            assert ((stack_new_1 + (0 - 7))%a = Some a2) as Hpop1.
+            { assert ((a3 + 1)%a = Some stack_own_b) as Hincr;[iContiguous_next Hcont1 2|].
+              assert ((a2 + 1)%a = Some a3) as Hincr';[iContiguous_next Hcont1 1|].
               revert Hstack_own_bound1' Hincr Hincr' Hstack_new_1. clear. solve_addr. }
             iApply (wp_lea_success_reg with "[$HPC $Hr_t1 $Hr_stk $Hinstr]");
               [apply lea_r_i|apply PermFlows_refl|iCorrectPC a27 a_last|
-               iContiguous_next Hcont_rest1 2|apply Hpop1|auto..].
+               iContiguous_next Hcont_rest2 2|apply Hpop1|auto..].
             iEpilogue "(HPC & Hinstr & Hr_t1 & Hr_stk)". iCombine "Hinstr" "Hprog_done" as "Hprog_done". 
             (* pop r_stk r_t0 *)
-            do 3 (destruct rest1; [inversion Hrest_length1|]).
-            iDestruct (big_sepL2_app_inv _ [a30;a31;a32] (a33::rest1) with "Hprog") as "[Hpop Hprog]";[simpl;auto|].
-            clear Hpop1. assert ((a3 + (0 - 1))%a = Some a2) as Hpop1.
-            { rewrite -(addr_add_assoc a2 _ 1);[apply addr_add_0|iContiguous_next Hcont1 0]. }
+            do 3 (destruct rest2; [inversion Hrest_length1|]).
+            iDestruct (big_sepL2_app_inv _ [a30;a31;a32] (a33::rest2) with "Hprog") as "[Hpop Hprog]";[simpl;auto|].
+            clear Hpop1. assert ((a2 + (0 - 1))%a = Some a0) as Hpop1.
+            { rewrite -(addr_add_assoc a0 _ 1);[apply addr_add_0|iContiguous_next Hcont1 0]. }
             iApply (pop_spec); [..|iFrame "HPC Hr_stk Hr_t1 Hpop Hr_t0 Ha3"];
-              [split;[|split];iCorrectPC a27 a_last|apply PermFlows_refl|iContiguous_bounds_withinBounds a2 stack_own_last|auto|iContiguous_next Hcont_rest1 3|iContiguous_next Hcont_rest1 4|iContiguous_next Hcont_rest1 5|apply Hpop1|].
+              [split;[|split];iCorrectPC a27 a_last|apply PermFlows_refl|iContiguous_bounds_withinBounds a0 stack_own_last|auto|iContiguous_next Hcont_rest2 3|iContiguous_next Hcont_rest2 4|iContiguous_next Hcont_rest2 5|apply Hpop1|].
             iNext. iIntros "(HPC & Hpop & Hr_t0 & Ha3 & Hr_stk & Hr_t1)". iCombine "Hpop" "Hprog_done" as "Hprog_done".
             (* pop r_stk r_env *)
-            do 3 (destruct rest1; [inversion Hrest_length1|]).
-            iDestruct (big_sepL2_app_inv _ [a33;a34;a35] (a36::rest1) with "Hprog") as "[Hpop Hprog]";[simpl;auto|].
-            clear Hpop1. assert ((a2 + (0 - 1))%a = Some b_r') as Hpop1.
+            do 3 (destruct rest2; [inversion Hrest_length1|]).
+            iDestruct (big_sepL2_app_inv _ [a33;a34;a35] (a36::rest2) with "Hprog") as "[Hpop Hprog]";[simpl;auto|].
+            clear Hpop1. assert ((a0 + (0 - 1))%a = Some b_r') as Hpop1.
             { revert Hb_r'. clear. solve_addr. }
             iApply (pop_spec); [..|iFrame "HPC Hr_stk Hr_t1 Hpop Hr_env Ha2"];
-              [split;[|split];iCorrectPC a27 a_last|apply PermFlows_refl|iContiguous_bounds_withinBounds a2 stack_own_last|auto|iContiguous_next Hcont_rest1 6|iContiguous_next Hcont_rest1 7|iContiguous_next Hcont_rest1 8|apply Hpop1|].
+              [split;[|split];iCorrectPC a27 a_last|apply PermFlows_refl|iContiguous_bounds_withinBounds a0 stack_own_last|auto|iContiguous_next Hcont_rest2 6|iContiguous_next Hcont_rest2 7|iContiguous_next Hcont_rest2 8|apply Hpop1|].
             iNext. iIntros "(HPC & Hpop & Hr_env & Ha2 & Hr_stk & Hr_t1)". iCombine "Hpop" "Hprog_done" as "Hprog_done".
             (* we have now arrived at the final load of the environment. we must here assert that the loaded
                value is indeed 1. We are able to show this since W6 is a public future world of W5, in which 
                invariant i is in state true *)
             (* load r_adv r_env *)
-            iPrologue rest1 Hrest_length1 "Hprog".
+            iPrologue rest2 Hrest_length1 "Hprog".
             iAssert (∀ φ, ▷ (PC ↦ᵣ inr (pc_p, pc_g, pc_b, pc_e, a37)
                                 ∗ r_env ↦ᵣ inr (RWX, Global, d, d', d)
                                 ∗ a36 ↦ₐ[pc_p] load_r r_adv r_env
@@ -2914,12 +3024,12 @@ Section awkward_example.
               iAssert (⌜(d =? a36)%a = false⌝)%I as %Hne.
               { destruct (d =? a36)%a eqn:Heq;auto. apply Z.eqb_eq,z_of_eq in Heq. rewrite Heq.
                 iDestruct (cap_duplicate_false with "[$Hinstr $Hb]") as "Hfalse";[|done].
-                eapply isCorrectPC_contiguous_range with (a := a0) in Hvpc;[|eauto|];last (by apply elem_of_cons;left). 
+                eapply isCorrectPC_contiguous_range with (a := a) in Hvpc;[|eauto|];last (by apply elem_of_cons;left). 
                 destruct pc_p;auto.
                 inversion Hvpc as [?????? [Hcontr | [Hcontr | Hcontr] ] ];inversion Hcontr. }
               iApply (wp_load_success with "[$HPC $Hinstr $Hr_adv $Hr_env Hb]");
                 [apply load_r_i|apply PermFlows_refl|iCorrectPC a27 a_last
-                 |auto|iContiguous_next Hcont_rest1 9|rewrite Hne;iFrame;iPureIntro;apply PermFlows_refl|rewrite Hne].
+                 |auto|iContiguous_next Hcont_rest2 9|rewrite Hne;iFrame;iPureIntro;apply PermFlows_refl|rewrite Hne].
               iNext. iIntros "(HPC & Hr_adv & Ha36 & Hr_env & Hd)".
               iMod ("Hcls" with "[Hstate Hd]") as "_".
               { iNext. iExists true. iFrame. }
@@ -2930,32 +3040,32 @@ Section awkward_example.
             iNext. iIntros "(HPC & Hr_env & Ha36 & Hsts & Hr_adv)".
             (* We can now assert that r_adv indeed points to 1 *)
             (* move r_t1 PC *)
-            iPrologue rest1 Hrest_length1 "Hprog". 
+            iPrologue rest2 Hrest_length1 "Hprog". 
             iApply (wp_move_success_reg_fromPC with "[$HPC $Hr_t1 $Hinstr]");
               [apply move_r_i|apply PermFlows_refl|iCorrectPC a27 a_last|
-               iContiguous_next Hcont_rest1 10|auto|..].
+               iContiguous_next Hcont_rest2 10|auto|..].
             iEpilogue "(HPC & Hinstr & Hr_t1)". iCombine "Hinstr" "Hprog_done" as "Hprog_done". 
             (* lea r_t1 5 *)
-            iPrologue rest1 Hrest_length1 "Hprog". 
-            do 2 (destruct rest1;[inversion Hrest_length1|]).
+            iPrologue rest2 Hrest_length1 "Hprog". 
+            do 2 (destruct rest2;[inversion Hrest_length1|]).
             assert ((a37 + 62)%a = Some a_last) as Hincr.
-            { revert Hcont_rest1 Hrest_length1. clear. intros Hcont_rest1 Hrest_length1.
+            { revert Hcont_rest2 Hrest_length1. clear. intros Hcont_rest1 Hrest_length1.
               assert ((a27 + 10)%a = Some a37);[eapply contiguous_between_incr_addr with (i:=10) (ai:=a37) in Hcont_rest1;auto|].
               apply contiguous_between_length in Hcont_rest1. solve_addr. }
             iApply (wp_lea_success_z with "[$HPC $Hinstr $Hr_t1]");
               [apply lea_z_i|apply PermFlows_refl|iCorrectPC a27 a_last|
-               iContiguous_next Hcont_rest1 11|apply Hincr|auto|..].
-            { apply isCorrectPC_range_npE in Hvpc; auto. revert Hf2;clear; intros H. apply contiguous_between_length in H. solve_addr. }
+               iContiguous_next Hcont_rest2 11|apply Hincr|auto|..].
+            { apply isCorrectPC_range_npE in Hvpc; auto. revert Hcont;clear; intros H. apply contiguous_between_length in H. solve_addr. }
             iEpilogue "(HPC & Hinstr & Hr_t1)". iCombine "Hinstr" "Hprog_done" as "Hprog_done". 
             (* sub r_adv r_adv 1 *)
             iDestruct "Hprog" as "[Hinstr Hprog]". iApply (wp_bind (fill [SeqCtx])).
             iApply (wp_add_sub_lt_success_dst_z with "[$HPC $Hinstr $Hr_adv]");
-              [apply sub_r_z_i|right;left;eauto|iContiguous_next Hcont_rest1 12|apply PermFlows_refl|iCorrectPC a27 a_last|..]. 
+              [apply sub_r_z_i|right;left;eauto|iContiguous_next Hcont_rest2 12|apply PermFlows_refl|iCorrectPC a27 a_last|..]. 
             iEpilogue "(HPC & Hinstr & Hr_adv)". iCombine "Hinstr" "Hprog_done" as "Hprog_done".
             (* jnz r_self *)
             iDestruct "Hprog" as "[Hinstr Hprog]". iApply (wp_bind (fill [SeqCtx])).
             iApply (wp_jnz_success_next with "[$HPC $Hinstr $Hr_t1 $Hr_adv]");
-              [apply jnz_i|apply PermFlows_refl|iCorrectPC a27 a_last|iContiguous_next Hcont_rest1 13|..].
+              [apply jnz_i|apply PermFlows_refl|iCorrectPC a27 a_last|iContiguous_next Hcont_rest2 13|..].
             iEpilogue "(HPC & Hinstr & Hr_t1 & Hr_adv)". iCombine "Hinstr" "Hprog_done" as "Hprog_done".  
             (* Since the assertion succeeded, we are now ready to jump back to the adv who called us *)
             (* Before we can return to the adversary, we must clear the local stack frame and registers. This will 
@@ -2963,28 +3073,28 @@ Section awkward_example.
                the full stack invariant *)
             (* we must prepare the stack capability so that we only clear the local stack frame *)
             (* getb r_t1 r_stk *)
-            iPrologue rest1 Hrest_length1 "Hprog". 
+            iPrologue rest2 Hrest_length1 "Hprog". 
             iApply (wp_Get_success with "[$HPC $Hinstr $Hr_stk $Hr_t1]");
-              [apply getb_i|auto|apply PermFlows_refl|iCorrectPC a27 a_last|iContiguous_next Hcont_rest1 14|auto..].
+              [apply getb_i|auto|apply PermFlows_refl|iCorrectPC a27 a_last|iContiguous_next Hcont_rest2 14|auto..].
             iEpilogue "(HPC & Hinstr & Hr_stk & Hr_t1)"; iSimpl in "Hr_t1"; iCombine "Hinstr" "Hprog_done" as "Hprog_done".
             (* add_r_z r_t2 r_t1 8 *)
-            iPrologue rest1 Hrest_length1 "Hprog".
+            iPrologue rest2 Hrest_length1 "Hprog".
             iApply (wp_add_sub_lt_success_r_z with "[$HPC $Hinstr $Hr_t2 $Hr_t1]");
-              [apply add_r_z_i|by left|iContiguous_next Hcont_rest1 15|apply PermFlows_refl|iCorrectPC a27 a_last|..].
+              [apply add_r_z_i|by left|iContiguous_next Hcont_rest2 15|apply PermFlows_refl|iCorrectPC a27 a_last|..].
             iEpilogue "(HPC & Hinstr & Hr_t1 & Hr_t2)"; iSimpl in "Hr_t2"; iCombine "Hinstr" "Hprog_done" as "Hprog_done". 
             (* subseg r_stk r_t1 r_t2 *)
-            assert (z_to_addr a2 = Some a2) as Ha2.
+            assert (z_to_addr a0 = Some a0) as Ha2.
             { rewrite /z_to_addr /=. clear. 
-              destruct (Z_le_dec a2 MemNum),(Z_le_dec 0 a2);destruct a2;
+              destruct (Z_le_dec a0 MemNum),(Z_le_dec 0 a0);destruct a0;
                 [f_equiv;by apply z_of_eq|zify_addr;apply Zle_bool_imp_le in pos..]. 
               lia. apply Zle_bool_imp_le in fin. lia. lia.               
             }
-            assert ((a2 + 10)%a = Some stack_own_end) as Ha2_stack_own_end.
-            { assert ((a2 + 3)%a = Some stack_own_b) as Ha2_stack_own_b.
+            assert ((a0 + 10)%a = Some stack_own_end) as Ha2_stack_own_end.
+            { assert ((a0 + 3)%a = Some stack_own_b) as Ha2_stack_own_b.
               { apply (contiguous_between_incr_addr _ 3 _ stack_own_b) in Hcont1; auto. }
               revert Ha2_stack_own_b Hstack_own_bound'. 
               clear; intros. solve_addr. }
-            assert (z_to_addr (a2 + 10)%Z = Some stack_own_end) as Ha2_stack_own_end'.
+            assert (z_to_addr (a0 + 10)%Z = Some stack_own_end) as Ha2_stack_own_end'.
             { (* fixme: very tedious *)
               revert Ha2_stack_own_end;clear. intros.
               destruct stack_own_end;simpl.
@@ -2997,33 +3107,33 @@ Section awkward_example.
               destruct (Z.leb_le 0 (z1 + 10)); try lia.
               repeat f_equal; apply eq_proofs_unicity; decide equality.
             }
-            iPrologue rest1 Hrest_length1 "Hprog".
+            iPrologue rest2 Hrest_length1 "Hprog".
             iApply (wp_subseg_success with "[$HPC $Hinstr $Hr_stk $Hr_t1 $Hr_t2]");
               [apply subseg_r_r_i|apply PermFlows_refl|iCorrectPC a27 a_last|
                split;[apply Ha2|apply Ha2_stack_own_end']|
-               auto|auto| |iContiguous_next Hcont_rest1 16|..].
+               auto|auto| |iContiguous_next Hcont_rest2 16|..].
             { rewrite !andb_true_iff !Z.leb_le. apply withinBounds_le_addr in Hwb2.
-              assert ((a2 + 3)%a = Some stack_own_b) as Ha2_stack_own_b.
+              assert ((a0 + 3)%a = Some stack_own_b) as Ha2_stack_own_b.
               { apply (contiguous_between_incr_addr _ 3 _ stack_own_b) in Hcont1; auto. }
               revert Hstack_own_bound Hwb2 Ha2_stack_own_end Ha2_stack_own_b.
               clear. repeat split; try lia; try solve_addr. }
             iEpilogue "(HPC & Hinstr & Hr_t1 & Hr_t2 & Hr_stk)". iCombine "Hinstr" "Hprog_done" as "Hprog_done".
-            iAssert ([[a2,stack_own_end]]↦ₐ[RWLX][[l_frame2]])%I with "[Hframe Ha2 Ha3]" as "Hstack".
+            iAssert ([[a0,stack_own_end]]↦ₐ[RWLX][[l_frame2]])%I with "[Hframe Ha2 Ha3]" as "Hstack".
             { iApply region_mapsto_cons;[iContiguous_next Hcont1 0|..].
-              { apply contiguous_between_middle_bounds with (i:=1) (ai:=a3) in Hcont1;auto.
+              { apply contiguous_between_middle_bounds with (i:=1) (ai:=a2) in Hcont1;auto.
                 revert Hstack_own_bound Hstack_own_bound' Hcont1;clear. solve_addr. }
               iFrame.
               iApply region_mapsto_cons;[iContiguous_next Hcont1 1|..].
-              { apply contiguous_between_middle_bounds with (i:=2) (ai:=a4) in Hcont1;auto.
+              { apply contiguous_between_middle_bounds with (i:=2) (ai:=a3) in Hcont1;auto.
                 revert Hstack_own_bound Hstack_own_bound' Hcont1;clear. solve_addr. }
               iFrame. 
             }
             (* We are now ready to clear the stack *)
-            assert (contiguous_between (a44 :: rest1) a44 a_last) as Hcont_weak.
-            { repeat (inversion Hcont_rest1 as [|????? Hf2']; subst; auto; clear Hcont_rest1; rename Hf2' into Hcont_rest1). }
+            assert (contiguous_between (a44 :: rest2) a44 a_last) as Hcont_weak.
+            { repeat (inversion Hcont_rest2 as [|????? Hcont_rest2']; subst; auto; clear Hcont_rest2; rename Hcont_rest2' into Hcont_rest2). }
             iDestruct (contiguous_between_program_split with "Hprog") as (mclear_addrs rclear_addrs rclear_first)
                                                                            "(Hmclear & Hrclear & #Hcont)"; [eauto|].
-            iDestruct "Hcont" as %(Hcont_mclear & Hcont_rest2 & Hstack_eq2 & Hlink2).
+            iDestruct "Hcont" as %(Hcont_mclear & Hcont_rest3 & Hstack_eq2 & Hlink3).
             iDestruct (big_sepL2_length with "Hmclear") as %Hmclear_length.
             assert (7 < (length mclear_addrs)) as Hlt7;[rewrite Hmclear_length /=;clear;lia|].
             assert (17 < (length mclear_addrs)) as Hlt17;[rewrite Hmclear_length /=;clear;lia|].
@@ -3033,10 +3143,10 @@ Section awkward_example.
             { rewrite (_: 10%Z = Z.of_nat (10 : nat)).
               eapply contiguous_between_incr_addr_middle; [eapply Hcont_mclear|..]. all: eauto. }
             assert (a44 < rclear_first)%a as Hcontlt2.
-            { revert Hmclear_length Hlink2. clear. solve_addr. }
+            { revert Hmclear_length Hlink3. clear. solve_addr. }
             assert (a27 <= a44)%a as Hcontge2.
             { apply region_addrs_of_contiguous_between in Hcont_scall1. subst.
-              revert Hscall_length1 Hcont_rest1 Hcontlt1 Hcontlt2. clear =>Hscall_length Hf2 Hcontlt Hcontlt2.
+              revert Hscall_length1 Hcont_rest2 Hcontlt1 Hcontlt2. clear =>Hscall_length Hf2 Hcontlt Hcontlt2.
               apply contiguous_between_middle_bounds with (i := 17) (ai := a44) in Hf2;[solve_addr|auto].
             }
             iGet_genpur_reg_map r3 r_t3 "Hmreg'" "Hfull3" "[Hr_t3 Hmreg']".
@@ -3045,12 +3155,11 @@ Section awkward_example.
             iGet_genpur_reg_map r3 r_t6 "Hmreg'" "Hfull3" "[Hr_t6 Hmreg']".
             iApply (mclear_spec with "[- $HPC $Hr_stk $Hstack $Hr_t1 $Hr_t2 $Hr_t3 $Hr_t4 $Hr_t5 $Hr_t6]");
               [apply Hcont_mclear|..]; eauto.
-            { assert (rclear_first <= a_last)%a as Hle;[by apply contiguous_between_bounds in Hcont_rest2|].
-              intros mid Hmid. apply isCorrectPC_inrange with a0 a_last; auto.
+            { assert (rclear_first <= a_last)%a as Hle;[by apply contiguous_between_bounds in Hcont_rest3|].
+              intros mid Hmid. apply isCorrectPC_inrange with link0 a_last; auto.
               revert Hle Hcontlt1 Hcontge1 Hcontlt Hcontge Hmid Hcontlt2 Hcontge2. clear; intros. split; try solve_addr.
             }
             { apply PermFlows_refl. }
-            { apply PermFlows_refl. } 
             { apply withinBounds_le_addr in Hwb3 as [? _]. auto. }
             rewrite /mclear.
             destruct (strings.length mclear_addrs =? strings.length (mclear_instrs r_stk 10 2))%nat eqn:Hcontr;
@@ -3086,13 +3195,13 @@ Section awkward_example.
             (* We are now ready to clear the registers *)
             iDestruct (big_sepL2_length with "Hrclear") as %Hrclear_length. 
             destruct rclear_addrs;[inversion Hrclear_length|].
-            apply contiguous_between_cons_inv_first in Hcont_rest2 as Heq. subst rclear_first.
+            apply contiguous_between_cons_inv_first in Hcont_rest3 as Heq. subst rclear_first.
             iDestruct (contiguous_between_program_split with "Hrclear") as (rclear jmp_addrs jmp_addr)
                                                                            "(Hrclear & Hjmp & #Hcont)"; [eauto|].
-            iDestruct "Hcont" as %(Hcont_rclear & Hcont_rest3 & Hstack_eq3 & Hlink3).
+            iDestruct "Hcont" as %(Hcont_rclear & Hcont_rest4 & Hstack_eq3 & Hlink4).
             clear Hrclear_length. iDestruct (big_sepL2_length with "Hrclear") as %Hrclear_length.
             assert (a45 < jmp_addr)%a as Hcontlt3.
-            { revert Hrclear_length Hlink3. clear. rewrite /all_registers /=. solve_addr. }
+            { revert Hrclear_length Hlink4. clear. rewrite /all_registers /=. solve_addr. }
             iAssert (⌜dom (gset RegName) r3 = all_registers_s⌝)%I as %Hdom_r3.
             { iDestruct "Hfull3" as %Hfull3. iPureIntro. apply (anti_symm _); [apply all_registers_subseteq|].
               rewrite elem_of_subseteq. intros ? _. rewrite -elem_of_gmap_dom. apply Hfull3. }
@@ -3100,8 +3209,8 @@ Section awkward_example.
             { eauto. }
             { apply not_elem_of_list; apply elem_of_cons; by left. }
             { destruct rclear; inversion Hcont_rclear; eauto. inversion Hrclear_length. }
-            { assert (jmp_addr <= a_last)%a as Hle;[by apply contiguous_between_bounds in Hcont_rest3|].
-              intros mid Hmid. apply isCorrectPC_inrange with a0 a_last; auto.
+            { assert (jmp_addr <= a_last)%a as Hle;[by apply contiguous_between_bounds in Hcont_rest4|].
+              intros mid Hmid. apply isCorrectPC_inrange with link0 a_last; auto.
               revert Hle Hcontlt1 Hcontge1 Hcontlt Hcontge Hmid Hcontlt2 Hcontge2 Hcontlt3. clear; intros. split; solve_addr.
             }
             { apply PermFlows_refl. }
@@ -3114,7 +3223,7 @@ Section awkward_example.
                are currently in a public future world of W *)
             assert (related_sts_pub_world W (std_update_multiple W6 (elements (dom (gset Addr) m_static2)) Temporary))
               as Hrelated7.
-            { eapply related_pub_local_3 with (b:=a2) (l1:=l') (l2:=l'');
+            { eapply related_pub_local_3 with (b:=a0) (l1:=l') (l2:=l'');
                 [..|apply Hrelated3|apply Hrelated6]; eauto; simpl; auto.
               - revert Hwb2 Hwb3. clear. intros Hwb2 Hwb3.
                 apply withinBounds_le_addr in Hwb2.
@@ -3130,7 +3239,7 @@ Section awkward_example.
                is a public future world of W3 *)
             assert (related_sts_pub_world W3 (std_update_multiple W6 (elements (dom (gset Addr) m_static2)) Temporary))
               as Hrelated8.
-            { eapply related_pub_local_4 with (b:=a2) (l1:=l') (l2:=l'');
+            { eapply related_pub_local_4 with (b:=a0) (l1:=l') (l2:=l'');
                 [..|apply Hrelated3|apply Hrelated6]; eauto; simpl; auto.
               - revert Hwb2 Hwb3. clear. intros Hwb2 Hwb3.
                 apply withinBounds_le_addr in Hwb2.
@@ -3152,17 +3261,17 @@ Section awkward_example.
                                       (std_update_multiple W6 (elements (dom (gset Addr) m_static2)) Temporary) φ0 a p'
                                       ∗ rel a p' φ0))%I.
               iApply (big_sepL2_to_static_region_perms _ _ ψ)%I;[auto|..]. 
-              { iAlways. iIntros (k a' pw Hpw1 Hpw2) "Hr". destruct pw. iFrame "Hr". }
+              { iAlways. iIntros (k a'' pw Hpw1 Hpw2) "Hr". destruct pw. iFrame "Hr". }
               iApply (big_sepL2_app with "[Hstack]").
               - iApply (big_sepL2_zip_repeat _ _ ψ).
                 iDestruct (region_addrs_zeroes_trans with "Hstack") as "Hstack".
                 rewrite (region_addrs_split _ stack_own_end).
-                iDestruct (big_sepL_app with "Hstack_val") as "[Hstack_val_frame _]".
+                iDestruct (big_sepL_app with "Hstack_region") as "[Hstack_val_frame _]".
                 iDestruct (big_sepL_sep with "[Hstack_val_frame Hstack]") as "Hstack".
                 iSplitL;[iFrame "Hstack"|iFrame "Hstack_val_frame"]. 
                 iDestruct (big_sepL2_to_big_sepL_l _ _ l_frame2 with "Hstack") as "Hstack";[auto|].
                 iApply (big_sepL2_mono with "Hstack"). 
-                iIntros (k a' _v Hy1 Yy2) "[Ha' Hrel]".
+                iIntros (k a'' _v Hy1 Yy2) "[Ha' [Hrel _] ]".
                 iExists RWLX,_v,(λ Wv : WORLD * Word, ((fixpoint interp1) Wv.1) Wv.2).
                 iSplit;[iPureIntro;apply _|]. iSplit;[auto|]. iFrame. iExists (inl 0%Z). iSimpl.
                 iSplit;[auto|]. iFrame. iSplit.
@@ -3177,10 +3286,10 @@ Section awkward_example.
                 { iSplitL;[iFrame "Hrest'"|iFrame "Hrest_valid'"]. }
                 iApply (big_sepL2_app with "[Hrest]").
                 + iApply (big_sepL2_mono with "Hrest").
-                  iIntros (k a' pw Ha' Hpw) "[Ha' Hr]".
+                  iIntros (k a'' pw Ha' Hpw) "[Ha' Hr]".
                   iDestruct "Hr" as (φ0 Hpers Hne) "(Hφ & Hrel & mono)".
-                  rewrite /ψ. destruct pw. simpl. iExists p,w17,φ0.
-                  repeat iSplit;auto. iExists w17. destruct (pwl p).
+                  rewrite /ψ. destruct pw. simpl. iExists p0,w17,φ0.
+                  repeat iSplit;auto. iExists w17. destruct (pwl p0).
                   { iDestruct "mono" as "#mono".
                     iAssert (φ0 (std_update_multiple W6 (elements (dom (gset Addr) m_static2)) Temporary, w17))
                       with "[Hφ]" as "Hφ".
@@ -3192,10 +3301,10 @@ Section awkward_example.
                     { iApply ("mono" with "[] Hφ"). iPureIntro. apply related_sts_pub_priv_world. auto. }
                     iFrame "∗ #". auto. }
                 + iApply (big_sepL2_mono with "Hrest'").
-                  iIntros (k a' pw Ha' Hpw) "[Ha' Hr]".
+                  iIntros (k a'' pw Ha' Hpw) "[Ha' Hr]".
                   iDestruct "Hr" as (φ0 Hpers Hne) "(Hφ & Hrel & mono)".
-                  rewrite /ψ. destruct pw. simpl. iExists p,w17,φ0.
-                  repeat iSplit;auto. iExists w17. destruct (pwl p).
+                  rewrite /ψ. destruct pw. simpl. iExists p0,w17,φ0.
+                  repeat iSplit;auto. iExists w17. destruct (pwl p0).
                   { iDestruct "mono" as "#mono".
                     iAssert (φ0 (std_update_multiple W6 (elements (dom (gset Addr) m_static2)) Temporary, w17))
                       with "[Hφ]" as "Hφ".
@@ -3210,6 +3319,29 @@ Section awkward_example.
 
             (* we can finish reasoning about the program *)
             rewrite /enter_cond /interp_expr /interp_conf. iSimpl in "Hcallback".
+            (* again we want to use the jump of fail pattern when jumping to unknown capabilities *)
+            iAssert (interp W wret) as "#Hcallback'";[|iClear "Hcallback"].
+            { rewrite fixpoint_interp1_eq. iFrame "Hcallback". }
+            iDestruct (jmp_or_fail_spec with "Hcallback'") as "Hcallback_now".
+
+            (* We can now finally jump to the return capability *)
+            (* jmp r_t0 *)
+            iDestruct (big_sepL2_length with "Hjmp") as %Hjmp_length.
+            destruct jmp_addrs; [inversion Hjmp_length|].
+            destruct jmp_addrs; [|inversion Hjmp_length].
+            apply contiguous_between_cons_inv_first in Hcont_rest4 as Heq; subst jmp_addr.
+            iDestruct "Hjmp" as "[Hinstr _]". iApply (wp_bind (fill [SeqCtx])).
+            iApply (wp_jmp_success with "[$HPC $Hinstr $Hr_t0]");
+              [apply jmp_i|apply PermFlows_refl|..].
+            { (* apply contiguous_between_bounds in Hcont_rest3 as Hle. *)
+              inversion Hcont_rest4 as [| a'' b' c' l3 Hnext Hcont_rest5 Heq Hnil Heq'].
+              inversion Hcont_rest5; subst. 
+              apply Hvpc2. revert Hcontge2 Hcontlt2 Hcontlt3 Hnext. clear. solve_addr. }
+
+            destruct (decide (isCorrectPC (updatePcPerm wret))).
+            2: { iEpilogue "(HPC & Hinstr & Hrt0)". iApply "Hcallback_now". iFrame. iIntros (Hcontr'). done. }
+            
+            iDestruct "Hcallback_now" as (p_ret g_ret b_ret e_ret a_ret Heqret) "Hcallback_now". simplify_eq. 
             iAssert (future_world g_ret W (std_update_multiple W6 (elements (dom (gset Addr) m_static2)) Temporary))%I
               as "#Hfuture". 
             { destruct g_ret; iSimpl.
@@ -3218,24 +3350,11 @@ Section awkward_example.
             }
             set r4 : gmap RegName Word :=
               <[PC := inl 0%Z]>
-              (<[r_t0 := inr (E, g_ret, b_ret, e_ret, a_ret)]>
+              (<[r_t0 := inr (p_ret, g_ret, b_ret, e_ret, a_ret)]>
               (create_gmap_default
                  (list_difference all_registers [PC; r_t0]) (inl 0%Z))).
-            iDestruct ("Hcallback" $! r4 with "Hfuture") as "Hcallback_now".
-
-            (* We can now finally jump to the return capability *)
-            (* jmp r_t0 *)
-            iDestruct (big_sepL2_length with "Hjmp") as %Hjmp_length.
-            destruct jmp_addrs; [inversion Hjmp_length|].
-            destruct jmp_addrs; [|inversion Hjmp_length].
-            apply contiguous_between_cons_inv_first in Hcont_rest3 as Heq; subst jmp_addr.
-            iDestruct "Hjmp" as "[Hinstr _]". iApply (wp_bind (fill [SeqCtx])).
-            iApply (wp_jmp_success with "[$HPC $Hinstr $Hr_t0]");
-              [apply jmp_i|apply PermFlows_refl|..].
-            { (* apply contiguous_between_bounds in Hcont_rest3 as Hle. *)
-              inversion Hcont_rest3 as [| a' b' c' l3 Hnext Hcont_rest4 Heq Hnil Heq'].
-              inversion Hcont_rest4; subst. 
-              apply Hvpc2. revert Hcontge2 Hcontlt2 Hcontlt3 Hnext. clear. solve_addr. }
+            iDestruct ("Hcallback_now" $! r4 with "Hfuture") as "Hcallback_now'".
+            
             iEpilogue "(HPC & Hinstr & Hrt0)". iCombine "Hinstr" "Hprog_done" as "Hprog_done". 
 
             
@@ -3257,7 +3376,7 @@ Section awkward_example.
             iSimpl in "HPC".
 
             (* we apply the callback to the current configuration *)
-            iSpecialize ("Hcallback_now" with "[Hsts Hr Hmreg' HPC Hrt0 Hna]"). 
+            iSpecialize ("Hcallback_now'" with "[Hsts Hr Hmreg' HPC Hrt0 Hna]"). 
             { iFrame "Hna Hr Hsts". iSplitR;[iSplit|].
               - iPureIntro. clear. 
                 intros x. rewrite /= /r4.
@@ -3270,12 +3389,12 @@ Section awkward_example.
                 rewrite /r4 lookup_insert_ne;auto.
                 destruct (decide (r_t0 = r0));[subst;rewrite lookup_insert|].
                 + iApply (interp_monotone $! Hrelated7).
-                  rewrite /interp /= fixpoint_interp1_eq /=. iFrame "Hcallback". 
+                  rewrite /interp fixpoint_interp1_eq. iFrame "Hcallback'". 
                 + rewrite lookup_insert_ne;[|auto]. 
                   assert (r0 ∈ (list_difference all_registers [PC; r_t0])) as Hin.
                   { apply elem_of_list_difference. split;[apply all_registers_correct|].
                     repeat (apply not_elem_of_cons; split;[auto|try apply not_elem_of_nil]). }
-                  rewrite fixpoint_interp1_eq. iRevert (Hin).
+                  rewrite !fixpoint_interp1_eq. iRevert (Hin).
                   rewrite (create_gmap_default_lookup _ (inl 0%Z : Word) r0).
                   iIntros (Hin). rewrite Hin. iSimpl. done. 
               - rewrite /registers_mapsto /r4 insert_insert.
@@ -3288,8 +3407,8 @@ Section awkward_example.
                 repeat rewrite ?dom_delete_L ?dom_insert_L. rewrite Hdom_r3.
                 rewrite !all_registers_union_l !difference_difference_L. f_equal. clear. set_solver.
             }
-            iDestruct "Hcallback_now" as "[_ Hcallback_now]".
-            iApply wp_wand_l. iFrame "Hcallback_now". 
+            iDestruct "Hcallback_now'" as "[_ Hcallback_now']".
+            iApply wp_wand_l. iFrame "Hcallback_now'". 
             iIntros (v) "Hv". 
             iIntros (halted). 
             iDestruct ("Hv" $! halted) as (r0 W0) "(#Hfull & Hmreg' & #Hrelated & Hna & Hsts & Hr)". 
@@ -3299,44 +3418,39 @@ Section awkward_example.
             eapply related_sts_priv_trans_world;[|apply Hrelated10].
             apply related_sts_pub_priv_world. 
             apply related_sts_pub_world_static_to_temporary with (m:=m_static2);auto.
-            apply Forall_forall. intros a' Hin. apply elem_of_elements in Hin. apply Hall_static' in Hin.
-            rewrite /static in Hin. destruct (W6.1 !! a') eqn:Hsome;[|done].
+            apply Forall_forall. intros a'' Hin. apply elem_of_elements in Hin. apply Hall_static' in Hin.
+            rewrite /static in Hin. destruct (W6.1 !! a'') eqn:Hsome;[|done].
             subst. auto. 
-          - rewrite Hr_t30. 
-            assert (r2 !! r_adv = Some (inr (E, Global, b, e, a))) as Hr_t30_some; auto. 
-            rewrite /RegLocate Hr_t30_some. repeat rewrite fixpoint_interp1_eq. iSimpl. 
-            iIntros (_). 
-            iAlways. rewrite /enter_cond.
-            iIntros (r0 W2 Hrelated2). 
-            iNext. iApply fundamental.
-            iLeft. done.
-            iExists RX. iSplit; auto.
-            iApply (adv_monotone with "Hadv_val"); auto.
+          - iAssert (interp W (inr (p, Global, b, e, a'))) as "#Hadv_val'";[|iClear "Hadv_val"].
+            { rewrite fixpoint_interp1_eq. iFrame "Hadv_val". }
+            rewrite Hr_t30. 
+            assert (r2 !! r_adv = Some (inr (p, Global, b, e, a'))) as Hr_t30_some; auto. 
+            rewrite /RegLocate Hr_t30_some. (* repeat rewrite fixpoint_interp1_eq. iSimpl.  *)
+            iIntros (_).
+            iApply (interp_monotone_nl with "[] [] Hadv_val'");[iPureIntro|auto].
             apply related_sts_priv_trans_world with W''; auto.
             eapply related_sts_priv_trans_world;[apply related_sts_pub_priv_world;apply Hrelated3|].
             apply related_sts_priv_trans_world with W5; auto.
+            apply related_sts_priv_refl_world. 
           - rewrite r_zero; auto.
             repeat rewrite fixpoint_interp1_eq. iPureIntro. auto.
         }
-        iDestruct ("Hvalid" with "[$Hsts $Hr $Hna $Hfull2 $Hmaps $Hreg]")
-          as "[_ Ho]". 
+        iDestruct ("Hadv_contW5" with "[$Hsts $Hr $Hna $Hfull2 $Hmaps $Hreg]")
+          as "[_ Ho]".
         iApply wp_wand_r. iFrame.
         iIntros (v) "Hhalted".
         iIntros (->).
-        iSpecialize ("Hhalted" with "[]");[auto|]. 
-        iDestruct "Hhalted" as (r0 W6) "(Hr0 & Hregr0 & % & Hna & Hsts)". 
-        iExists _,_. iFrame. 
-        iPureIntro. eapply related_sts_priv_trans_world;[apply Hrelated5|auto]. 
+        iSpecialize ("Hhalted" with "[]");[auto|].
+        iDestruct "Hhalted" as (r0 W6) "(Hr0 & Hregr0 & % & Hna & Hsts)".
+        iExists _,_. iFrame.
+        iPureIntro. eapply related_sts_priv_trans_world;[apply Hrelated5|auto].
       - rewrite Hr_t30. 
-        assert (r !! r_adv = Some (inr (E, Global, b, e, a))) as Hr_t30_some; auto. 
-        rewrite /RegLocate Hr_t30_some fixpoint_interp1_eq. iSimpl. 
+        assert (r !! r_adv = Some (inr (p, Global, b, e, a'))) as Hr_t30_some; auto. 
+        rewrite /RegLocate Hr_t30_some. iSimpl. 
         iIntros (_). 
-        iAlways. iIntros (r' W3 Hrelated3). 
-        iNext. iApply fundamental.
-        iLeft. done.
-        iExists RX. iSplit; simpl; auto.
-        iApply (adv_monotone with "Hadv_val");auto.
-        eapply related_sts_priv_trans_world;[apply HWW''|auto].          
+        iApply (interp_monotone_nl with "[] [] Hadv_val");[iPureIntro|auto].
+        eapply related_sts_priv_trans_world;[apply HWW''|auto].
+        apply related_sts_priv_refl_world. 
       - (* in this case we can infer that r1 points to 0, since it is in the list diff *)
         iIntros (Hne). 
         assert (r !r! r1 = inl 0%Z) as Hr1.
@@ -3351,11 +3465,11 @@ Section awkward_example.
           }
             by inversion Heq. 
         }
-        rewrite Hr1 fixpoint_interp1_eq. iPureIntro. eauto.         
+        rewrite Hr1 !fixpoint_interp1_eq. auto. 
     }
     iAssert (((interp_reg interp) W'' r))%I as "#HvalR";[iSimpl;auto|]. 
-    iSpecialize ("Hvalid" with "[$HvalR $Hmaps Hsts $Hna $Hr]"); iFrame. 
-    iDestruct "Hvalid" as "[_ Ho]". 
+    iSpecialize ("Hadv_contW''" with "[$HvalR $Hmaps Hsts $Hna $Hr]"); iFrame. 
+    iDestruct "Hadv_contW''" as "[_ Ho]". 
     rewrite /interp_conf.
     iApply wp_wand_r. iFrame.
     iIntros (v) "Htest".
